rename substs

Superposition_Calculus/First_Order_Superposition.thy
@@ -18,7 +18,7 @@ section \<open>First-Order Layer\<close>
 
 definition clause_groundings ::
   "('f, 'v) atom clause \<Rightarrow> 'f ground_atom clause set" where
-  "clause_groundings clause = { to_ground_clause (clause \<cdot> \<theta>) | \<theta>. is_ground_clause (clause \<cdot> \<theta>) }"
+  "clause_groundings clause = { to_ground_clause (clause \<cdot> \<gamma>) | \<gamma>. is_ground_clause (clause \<cdot> \<gamma>) }"
 
 locale first_order_superposition_calculus =
   first_order_select select +
