Superposition_Calculus/First_Order_Superposition_Completeness.thy
@@ -12,20 +12,20 @@ lemma eq_resolution_lifting:
   fixes 
     premise\<^sub>G conclusion\<^sub>G :: "'f gatom clause" and 
     premise conclusion :: "('f, 'v) atom clause" and
-    \<theta> :: "('f, 'v) subst"
+    \<gamma> :: "('f, 'v) subst"
   defines 
-    premise\<^sub>G [simp]: "premise\<^sub>G \<equiv> to_ground_clause (premise \<cdot> \<theta>)" and
-    conclusion\<^sub>G [simp]: "conclusion\<^sub>G \<equiv> to_ground_clause (conclusion \<cdot> \<theta>)"
+    premise\<^sub>G [simp]: "premise\<^sub>G \<equiv> to_ground_clause (premise \<cdot> \<gamma>)" and
+    conclusion\<^sub>G [simp]: "conclusion\<^sub>G \<equiv> to_ground_clause (conclusion \<cdot> \<gamma>)"
   assumes 
-    premise_grounding [intro]: "is_ground_clause (premise \<cdot> \<theta>)" and
-    conclusion_grounding [intro]: "is_ground_clause (conclusion \<cdot> \<theta>)" and
-    select: "to_clause (select\<^sub>G premise\<^sub>G) = (select premise) \<cdot> \<theta>" and
-    ground_eq_resolution:  "ground.ground_eq_resolution premise\<^sub>G conclusion\<^sub>G"
+    premise_grounding [intro]: "is_ground_clause (premise \<cdot> \<gamma>)" and
+    conclusion_grounding [intro]: "is_ground_clause (conclusion \<cdot> \<gamma>)" and
+    select: "to_clause (select\<^sub>G premise\<^sub>G) = (select premise) \<cdot> \<gamma>" and
+    ground_eq_resolution: "ground.ground_eq_resolution premise\<^sub>G conclusion\<^sub>G"
   obtains conclusion' 
   where
     "eq_resolution premise conclusion'"
     "Infer [premise\<^sub>G] conclusion\<^sub>G \<in> inference_groundings (Infer [premise] conclusion')"
-    "conclusion' \<cdot> \<theta> = conclusion \<cdot> \<theta>"
+    "conclusion' \<cdot> \<gamma> = conclusion \<cdot> \<gamma>"
   using ground_eq_resolution
 proof(cases premise\<^sub>G conclusion\<^sub>G rule: ground.ground_eq_resolution.cases)
   case (ground_eq_resolutionI literal\<^sub>G premise\<^sub>G' term\<^sub>G)
@@ -38,58 +38,61 @@ proof(cases premise\<^sub>G conclusion\<^sub>G rule: ground.ground_eq_resolution
     unfolding premise\<^sub>G
     by (metis to_clause_empty_mset to_clause_inverse)
 
-  have "premise \<cdot> \<theta> = to_clause (add_mset literal\<^sub>G (to_ground_clause (conclusion \<cdot> \<theta>)))"
+  have "premise \<cdot> \<gamma> = to_clause (add_mset literal\<^sub>G (to_ground_clause (conclusion \<cdot> \<gamma>)))"
     using 
       ground_eq_resolutionI(1)[THEN arg_cong, of to_clause]
       to_ground_clause_inverse[OF premise_grounding]
-    unfolding premise\<^sub>G
-    using \<open>conclusion\<^sub>G = premise\<^sub>G'\<close> conclusion\<^sub>G
+      ground_eq_resolutionI(4)
+    unfolding premise\<^sub>G conclusion\<^sub>G
     by metis
 
-  also have "... = add_mset (to_literal literal\<^sub>G) (conclusion \<cdot> \<theta>)"
+  also have "... = add_mset (to_literal literal\<^sub>G) (conclusion \<cdot> \<gamma>)"
     unfolding to_clause_add_mset
     by (simp add: conclusion_grounding)
 
-  finally have premise': "premise \<cdot> \<theta> = add_mset (to_literal literal\<^sub>G) (conclusion \<cdot> \<theta>)".
+  finally have premise_\<gamma> : "premise \<cdot> \<gamma> = add_mset (to_literal literal\<^sub>G) (conclusion \<cdot> \<gamma>)".
 
-  let ?select\<^sub>G_empty = "select\<^sub>G (to_ground_clause (premise \<cdot> \<theta>)) = {#}"
-  let ?select\<^sub>G_not_empty = "select\<^sub>G (to_ground_clause (premise \<cdot> \<theta>)) \<noteq> {#}"
+  let ?select\<^sub>G_empty = "select\<^sub>G premise\<^sub>G = {#}"
+  let ?select\<^sub>G_not_empty = "select\<^sub>G premise\<^sub>G \<noteq> {#}"
 
   obtain max_literal where max_literal: 
     "is_maximal\<^sub>l max_literal premise" 
-    "is_maximal\<^sub>l (max_literal \<cdot>l \<theta>) (premise \<cdot> \<theta>)"
+    "is_maximal\<^sub>l (max_literal \<cdot>l \<gamma>) (premise \<cdot> \<gamma>)"
     using is_maximal\<^sub>l_ground_subst_stability[OF premise_not_empty premise_grounding]
     by blast
 
   moreover then have "max_literal \<in># premise"
     using maximal\<^sub>l_in_clause by fastforce
 
-  moreover have max_literal_literal\<^sub>G: 
-    "max_literal \<cdot>l \<theta> = to_literal (term\<^sub>G !\<approx> term\<^sub>G)"
-    if ?select\<^sub>G_empty
+  moreover have max_literal_\<gamma>: 
+    "max_literal \<cdot>l \<gamma> = to_literal (term\<^sub>G !\<approx> term\<^sub>G)"
+  if ?select\<^sub>G_empty
     using ground_eq_resolutionI(3) max_literal unique_maximal_in_ground_clause
     unfolding ground_eq_resolutionI(2) is_maximal_lit_iff_is_maximal\<^sub>l premise\<^sub>G
-    by (metis empty_not_add_mset maximal\<^sub>l_in_clause multi_member_split premise_grounding that to_clause_empty_mset to_ground_clause_inverse)
-
+    by (metis add_mset_not_empty maximal\<^sub>l_in_clause multi_member_split premise\<^sub>G premise_grounding 
+          that to_clause_empty_mset to_ground_clause_inverse)
+  
   moreover obtain selected_literal where 
-    "selected_literal \<cdot>l \<theta> = to_literal (term\<^sub>G !\<approx> term\<^sub>G)" and
+    "selected_literal \<cdot>l \<gamma> = to_literal (term\<^sub>G !\<approx> term\<^sub>G)" and
     "is_maximal\<^sub>l selected_literal (select premise)" 
   if ?select\<^sub>G_not_empty
     using ground_eq_resolutionI(3) select
     unfolding ground_eq_resolutionI(2) premise\<^sub>G
-    by (metis clause_subst_empty(2) is_maximal\<^sub>l_ground_subst_stability is_maximal_lit_iff_is_maximal\<^sub>l premise_grounding select_subst1 to_clause_inverse to_ground_clause_empty_mset unique_maximal_in_ground_clause)
+    by (metis clause_subst_empty(2) is_maximal\<^sub>l_ground_subst_stability 
+          is_maximal_lit_iff_is_maximal\<^sub>l premise_grounding select_subst1 to_clause_inverse 
+          to_ground_clause_empty_mset unique_maximal_in_ground_clause)
 
   moreover then have "?select\<^sub>G_not_empty \<Longrightarrow> selected_literal \<in># premise"
     by (meson maximal\<^sub>l_in_clause mset_subset_eqD select_subset)
 
   ultimately obtain literal where
-    literal: "literal \<cdot>l \<theta> = to_literal (term\<^sub>G !\<approx> term\<^sub>G)" and
+    literal: "literal \<cdot>l \<gamma> = to_literal (term\<^sub>G !\<approx> term\<^sub>G)" and
     literal_in_premise: "literal \<in># premise" and
     literal_selected: "?select\<^sub>G_not_empty \<Longrightarrow> is_maximal\<^sub>l literal (select premise)" and
     literal_max: "?select\<^sub>G_empty \<Longrightarrow> is_maximal\<^sub>l literal premise"
     by blast    
 
-  have literal_grounding: "is_ground_literal (literal \<cdot>l \<theta>)"
+  have literal_grounding: "is_ground_literal (literal \<cdot>l \<gamma>)"
     using literal ground_literal_is_ground
     by simp
 
@@ -97,18 +100,18 @@ proof(cases premise\<^sub>G conclusion\<^sub>G rule: ground.ground_eq_resolution
     using subst_polarity_stable to_literal_polarity_stable
     by (metis literal.collapse(2) literal.disc(2) uprod_exhaust)
 
-  have term_term': "term \<cdot>t \<theta> = term' \<cdot>t \<theta>"
+  have term_term': "term \<cdot>t \<gamma> = term' \<cdot>t \<gamma>"
     using literal
     unfolding terms subst_literal(2) subst_atom_def to_literal_def to_atom_def
     by simp
 
-  then obtain \<sigma> \<tau> where \<sigma>: "term_subst.is_imgu \<sigma> {{term, term'}}" "\<theta> = \<sigma> \<odot> \<tau>"
+  then obtain \<mu> \<sigma> where \<mu>: "term_subst.is_imgu \<mu> {{term, term'}}" "\<gamma> = \<mu> \<odot> \<sigma>"
     using imgu_exists
     by blast
 
   have literal\<^sub>G: 
-    "to_literal literal\<^sub>G = (term !\<approx> term') \<cdot>l \<theta>" 
-    "literal\<^sub>G = to_ground_literal ((term !\<approx> term') \<cdot>l \<theta>)"
+    "to_literal literal\<^sub>G = (term !\<approx> term') \<cdot>l \<gamma>" 
+    "literal\<^sub>G = to_ground_literal ((term !\<approx> term') \<cdot>l \<gamma>)"
     using literal ground_eq_resolutionI(2)  terms 
     by simp_all
 
@@ -116,12 +119,12 @@ proof(cases premise\<^sub>G conclusion\<^sub>G rule: ground.ground_eq_resolution
     using multi_member_split[OF literal_in_premise]
     by blast
 
-  have conclusion'_\<theta>: "conclusion' \<cdot> \<theta> = conclusion \<cdot> \<theta>"
-    using premise'
+  have conclusion'_\<gamma>: "conclusion' \<cdot> \<gamma> = conclusion \<cdot> \<gamma>"
+    using premise_\<gamma>
     unfolding conclusion' ground_eq_resolutionI(2) literal[symmetric] subst_clause_add_mset
     by simp
 
-  have eq_resolution: "eq_resolution premise (conclusion' \<cdot> \<sigma>)"
+  have eq_resolution: "eq_resolution premise (conclusion' \<cdot> \<mu>)"
   proof (rule eq_resolutionI)
     show "premise = add_mset literal conclusion'"
       using conclusion'.
@@ -129,28 +132,28 @@ proof(cases premise\<^sub>G conclusion\<^sub>G rule: ground.ground_eq_resolution
     show "literal = term !\<approx> term'"
       using terms.    
   next
-    show "term_subst.is_imgu \<sigma> {{term, term'}}"
-      using \<sigma>(1).
+    show "term_subst.is_imgu \<mu> {{term, term'}}"
+      using \<mu>(1).
   next
-    show "select premise = {#} \<and> is_maximal\<^sub>l (literal \<cdot>l \<sigma>) (premise \<cdot> \<sigma>) 
+    show "select premise = {#} \<and> is_maximal\<^sub>l (literal \<cdot>l \<mu>) (premise \<cdot> \<mu>) 
        \<or>  is_maximal\<^sub>l literal (select premise)"
     proof(cases ?select\<^sub>G_empty)
       case select\<^sub>G_empty: True
 
-      then have "max_literal \<cdot>l \<theta> = literal \<cdot>l \<theta>"
-        by (simp add: max_literal_literal\<^sub>G literal)
+      then have "max_literal \<cdot>l \<gamma> = literal \<cdot>l \<gamma>"
+        by (simp add: max_literal_\<gamma> literal)
 
-      then have literal_\<theta>_is_maximal: "is_maximal\<^sub>l (literal \<cdot>l \<theta>) (premise \<cdot> \<theta>)"
+      then have literal_\<gamma>_is_maximal: "is_maximal\<^sub>l (literal \<cdot>l \<gamma>) (premise \<cdot> \<gamma>)"
         using max_literal(2) by simp
 
-      have literal_\<sigma>_in_premise: "literal \<cdot>l \<sigma> \<in># premise \<cdot> \<sigma>"
+      have literal_\<mu>_in_premise: "literal \<cdot>l \<mu> \<in># premise \<cdot> \<mu>"
         by (simp add: literal_in_clause_subst literal_in_premise)
 
-      have "is_maximal\<^sub>l (literal \<cdot>l \<sigma>) (premise \<cdot> \<sigma>)"
+      have "is_maximal\<^sub>l (literal \<cdot>l \<mu>) (premise \<cdot> \<mu>)"
         using is_maximal\<^sub>l_ground_subst_stability'[OF 
-            literal_\<sigma>_in_premise 
-            premise_grounding[unfolded \<sigma>(2) clause_subst_compose]
-            literal_\<theta>_is_maximal[unfolded \<sigma>(2) clause_subst_compose literal_subst_compose]
+            literal_\<mu>_in_premise 
+            premise_grounding[unfolded \<mu>(2) clause_subst_compose]
+            literal_\<gamma>_is_maximal[unfolded \<mu>(2) clause_subst_compose literal_subst_compose]
             ].
 
       then show ?thesis
@@ -162,24 +165,24 @@ proof(cases premise\<^sub>G conclusion\<^sub>G rule: ground.ground_eq_resolution
         using literal_selected by blast
     qed
   next 
-    show "conclusion' \<cdot> \<sigma> = conclusion' \<cdot> \<sigma>" ..
+    show "conclusion' \<cdot> \<mu> = conclusion' \<cdot> \<mu>" ..
   qed
 
-  have "term_subst.is_idem \<sigma>"
-    using \<sigma>(1)
+  have "term_subst.is_idem \<mu>"
+    using \<mu>(1)
     by (simp add: term_subst.is_imgu_iff_is_idem_and_is_mgu)  
 
-  then have \<sigma>_\<theta>: "\<sigma> \<odot> \<theta> = \<theta>"
-    unfolding \<sigma>(2) term_subst.is_idem_def
+  then have \<mu>_\<gamma>: "\<mu> \<odot> \<gamma> = \<gamma>"
+    unfolding \<mu>(2) term_subst.is_idem_def
     by (metis subst_compose_assoc)
 
-  have conclusion'_\<sigma>_\<theta> : "conclusion' \<cdot> \<sigma> \<cdot> \<theta> = conclusion \<cdot> \<theta>"
-    using conclusion'_\<theta>  
-    unfolding clause_subst_compose[symmetric] \<sigma>_\<theta>.
+  have conclusion'_\<mu>_\<gamma> : "conclusion' \<cdot> \<mu> \<cdot> \<gamma> = conclusion \<cdot> \<gamma>"
+    using conclusion'_\<gamma>  
+    unfolding clause_subst_compose[symmetric] \<mu>_\<gamma>.
 
-  have "to_ground_clause (conclusion \<cdot> \<theta>) \<in> clause_groundings (conclusion' \<cdot> \<sigma>)"
-    unfolding clause_groundings_def conclusion'_\<sigma>_\<theta>
-    by (smt (verit, ccfv_threshold) conclusion'_\<sigma>_\<theta> conclusion_grounding mem_Collect_eq)
+  have "to_ground_clause (conclusion \<cdot> \<gamma>) \<in> clause_groundings (conclusion' \<cdot> \<mu>)"
+    unfolding clause_groundings_def conclusion'_\<mu>_\<gamma>
+    by (smt (verit, ccfv_threshold) conclusion'_\<mu>_\<gamma> conclusion_grounding mem_Collect_eq)
 
 (* TODO *)
   with eq_resolution that
@@ -193,27 +196,27 @@ proof(cases premise\<^sub>G conclusion\<^sub>G rule: ground.ground_eq_resolution
 
     using premise_grounding 
     apply auto
-    by (metis conclusion'_\<sigma>_\<theta> conclusion_grounding ground_eq_resolution premise\<^sub>G conclusion\<^sub>G)
+    by (metis conclusion'_\<mu>_\<gamma> conclusion_grounding ground_eq_resolution premise\<^sub>G conclusion\<^sub>G)
 qed
 
 lemma eq_factoring_lifting:
   fixes 
     premise\<^sub>G conclusion\<^sub>G :: "'f gatom clause" and 
     premise conclusion :: "('f, 'v) atom clause" and
-    \<theta> :: "('f, 'v) subst"
+    \<gamma> :: "('f, 'v) subst"
   defines 
-    premise\<^sub>G [simp]: "premise\<^sub>G \<equiv> to_ground_clause (premise \<cdot> \<theta>)" and
-    conclusion\<^sub>G [simp]: "conclusion\<^sub>G \<equiv> to_ground_clause (conclusion \<cdot> \<theta>)"
+    premise\<^sub>G [simp]: "premise\<^sub>G \<equiv> to_ground_clause (premise \<cdot> \<gamma>)" and
+    conclusion\<^sub>G [simp]: "conclusion\<^sub>G \<equiv> to_ground_clause (conclusion \<cdot> \<gamma>)"
   assumes
-    premise_grounding [intro]: "is_ground_clause (premise \<cdot> \<theta>)" and
-    conclusion_grounding [intro]: "is_ground_clause (conclusion \<cdot> \<theta>)" and
-    select: "to_clause (select\<^sub>G premise\<^sub>G) = (select premise) \<cdot> \<theta>" and
+    premise_grounding [intro]: "is_ground_clause (premise \<cdot> \<gamma>)" and
+    conclusion_grounding [intro]: "is_ground_clause (conclusion \<cdot> \<gamma>)" and
+    select: "to_clause (select\<^sub>G premise\<^sub>G) = (select premise) \<cdot> \<gamma>" and
     ground_eq_factoring: "ground.ground_eq_factoring premise\<^sub>G conclusion\<^sub>G"
   obtains conclusion' 
   where
     "eq_factoring premise (conclusion')"
     "Infer [premise\<^sub>G] conclusion\<^sub>G \<in> inference_groundings (Infer [premise] conclusion')"
-    "conclusion' \<cdot> \<theta> = conclusion \<cdot> \<theta>"
+    "conclusion' \<cdot> \<gamma> = conclusion \<cdot> \<gamma>"
   using ground_eq_factoring
 proof(cases premise\<^sub>G conclusion\<^sub>G rule: ground.ground_eq_factoring.cases)
   case (ground_eq_factoringI literal\<^sub>G\<^sub>1 literal\<^sub>G\<^sub>2 premise'\<^sub>G term\<^sub>G\<^sub>1 term\<^sub>G\<^sub>2 term\<^sub>G\<^sub>3)
@@ -226,13 +229,13 @@ proof(cases premise\<^sub>G conclusion\<^sub>G rule: ground.ground_eq_factoring.
     using ground_eq_factoringI(4) select clause_subst_empty
     by auto
 
-  have premise_\<theta>: "premise \<cdot> \<theta> = to_clause (add_mset literal\<^sub>G\<^sub>1 (add_mset literal\<^sub>G\<^sub>2 premise'\<^sub>G))"
+  have premise_\<gamma>: "premise \<cdot> \<gamma> = to_clause (add_mset literal\<^sub>G\<^sub>1 (add_mset literal\<^sub>G\<^sub>2 premise'\<^sub>G))"
     using ground_eq_factoringI(1) premise\<^sub>G
     by (metis premise_grounding to_ground_clause_inverse)
 
   obtain literal\<^sub>1 where literal\<^sub>1_maximal: 
     "is_maximal\<^sub>l literal\<^sub>1 premise" 
-    "is_maximal\<^sub>l (literal\<^sub>1 \<cdot>l \<theta>) (premise \<cdot> \<theta>)"
+    "is_maximal\<^sub>l (literal\<^sub>1 \<cdot>l \<gamma>) (premise \<cdot> \<gamma>)"
     using is_maximal\<^sub>l_ground_subst_stability[OF premise_not_empty premise_grounding]
     by blast
 
@@ -242,7 +245,7 @@ proof(cases premise\<^sub>G conclusion\<^sub>G rule: ground.ground_eq_factoring.
       unfolded ground_eq_factoringI(2) to_ground_clause_inverse[OF premise_grounding] premise\<^sub>G
       ]
 
-  have literal\<^sub>1: "literal\<^sub>1 \<cdot>l \<theta> = to_literal literal\<^sub>G\<^sub>1"
+  have literal\<^sub>1: "literal\<^sub>1 \<cdot>l \<gamma> = to_literal literal\<^sub>G\<^sub>1"
     using 
       unique_maximal_in_ground_clause[OF premise_grounding literal\<^sub>1_maximal(2) max_ground_literal]
       ground_eq_factoringI(2)
@@ -255,7 +258,7 @@ proof(cases premise\<^sub>G conclusion\<^sub>G rule: ground.ground_eq_factoring.
 
   with literal\<^sub>1 obtain term\<^sub>1 term\<^sub>1' where 
     literal\<^sub>1_terms: "literal\<^sub>1 = term\<^sub>1 \<approx> term\<^sub>1'" and
-    term\<^sub>G\<^sub>1_term\<^sub>1: "to_term term\<^sub>G\<^sub>1 = term\<^sub>1 \<cdot>t \<theta>"
+    term\<^sub>G\<^sub>1_term\<^sub>1: "to_term term\<^sub>G\<^sub>1 = term\<^sub>1 \<cdot>t \<gamma>"
     unfolding ground_eq_factoringI(2) to_literal_def to_atom_def subst_literal_def subst_atom_def 
     by force 
 
@@ -263,13 +266,13 @@ proof(cases premise\<^sub>G conclusion\<^sub>G rule: ground.ground_eq_factoring.
     using maximal\<^sub>l_in_clause[OF literal\<^sub>1_maximal(1)]
     by (meson multi_member_split)
 
-  then have premise''_\<theta>: "premise'' \<cdot> \<theta> =  add_mset (to_literal literal\<^sub>G\<^sub>2) (to_clause premise'\<^sub>G)"
-    using premise_\<theta> 
+  then have premise''_\<gamma>: "premise'' \<cdot> \<gamma> =  add_mset (to_literal literal\<^sub>G\<^sub>2) (to_clause premise'\<^sub>G)"
+    using premise_\<gamma> 
     unfolding to_clause_add_mset literal\<^sub>1[symmetric]
     by (simp add: subst_clause_add_mset)
 
   then obtain literal\<^sub>2 where literal\<^sub>2:
-    "literal\<^sub>2 \<cdot>l \<theta> = to_literal literal\<^sub>G\<^sub>2"
+    "literal\<^sub>2 \<cdot>l \<gamma> = to_literal literal\<^sub>G\<^sub>2"
     "literal\<^sub>2 \<in># premise''"
     unfolding subst_clause_def
     using msed_map_invR by force
@@ -281,19 +284,19 @@ proof(cases premise\<^sub>G conclusion\<^sub>G rule: ground.ground_eq_factoring.
 
   with literal\<^sub>2 obtain term\<^sub>2 term\<^sub>2' where 
     literal\<^sub>2_terms: "literal\<^sub>2 = term\<^sub>2 \<approx> term\<^sub>2'" and
-    term\<^sub>G\<^sub>1_term\<^sub>2: "to_term term\<^sub>G\<^sub>1 = term\<^sub>2 \<cdot>t \<theta>"
+    term\<^sub>G\<^sub>1_term\<^sub>2: "to_term term\<^sub>G\<^sub>1 = term\<^sub>2 \<cdot>t \<gamma>"
     unfolding ground_eq_factoringI(3) to_literal_def to_atom_def subst_literal_def subst_atom_def 
     by force
 
-  have term\<^sub>1_term\<^sub>2: "term\<^sub>1 \<cdot>t \<theta> = term\<^sub>2 \<cdot>t \<theta>"
+  have term\<^sub>1_term\<^sub>2: "term\<^sub>1 \<cdot>t \<gamma> = term\<^sub>2 \<cdot>t \<gamma>"
     using term\<^sub>G\<^sub>1_term\<^sub>1 term\<^sub>G\<^sub>1_term\<^sub>2
     by argo
 
-  then obtain \<sigma> \<tau> where \<sigma>: "term_subst.is_imgu \<sigma> {{term\<^sub>1, term\<^sub>2}}" "\<theta> = \<sigma> \<odot> \<tau>"
+  then obtain \<mu> \<sigma> where \<mu>: "term_subst.is_imgu \<mu> {{term\<^sub>1, term\<^sub>2}}" "\<gamma> = \<mu> \<odot> \<sigma>"
     using imgu_exists
     by blast
 
-  have term\<^sub>G\<^sub>2_term\<^sub>1': "to_term term\<^sub>G\<^sub>2 = term\<^sub>1' \<cdot>t \<theta>"
+  have term\<^sub>G\<^sub>2_term\<^sub>1': "to_term term\<^sub>G\<^sub>2 = term\<^sub>1' \<cdot>t \<gamma>"
     using literal\<^sub>1 term\<^sub>G\<^sub>1_term\<^sub>1 
     unfolding 
       literal\<^sub>1_terms 
@@ -304,7 +307,7 @@ proof(cases premise\<^sub>G conclusion\<^sub>G rule: ground.ground_eq_factoring.
       subst_atom_def 
     by auto
 
-  have term\<^sub>G\<^sub>3_term\<^sub>2': "to_term term\<^sub>G\<^sub>3 = term\<^sub>2' \<cdot>t \<theta>"
+  have term\<^sub>G\<^sub>3_term\<^sub>2': "to_term term\<^sub>G\<^sub>3 = term\<^sub>2' \<cdot>t \<gamma>"
     using literal\<^sub>2 term\<^sub>G\<^sub>1_term\<^sub>2
     unfolding 
       literal\<^sub>2_terms 
@@ -319,14 +322,14 @@ proof(cases premise\<^sub>G conclusion\<^sub>G rule: ground.ground_eq_factoring.
     using literal\<^sub>2(2) maximal\<^sub>l_in_clause[OF  literal\<^sub>1_maximal(1)] premise''
     by (metis multi_member_split)
 
-  then have premise'_\<theta>: "premise' \<cdot> \<theta> = to_clause premise'\<^sub>G"
-    using premise''_\<theta>  premise''
+  then have premise'_\<gamma>: "premise' \<cdot> \<gamma> = to_clause premise'\<^sub>G"
+    using premise''_\<gamma>  premise''
     unfolding literal\<^sub>2(1)[symmetric]
     by (simp add: subst_clause_add_mset)
 
   let ?conclusion' = "add_mset (term\<^sub>1 \<approx> term\<^sub>2') (add_mset (term\<^sub>1' !\<approx> term\<^sub>2') premise')"
 
-  have eq_factoring: "eq_factoring premise (?conclusion' \<cdot> \<sigma>)"
+  have eq_factoring: "eq_factoring premise (?conclusion' \<cdot> \<mu>)"
   proof (rule eq_factoringI)
     show "premise = add_mset literal\<^sub>1 (add_mset literal\<^sub>2 premise')"
       using premise.
@@ -340,117 +343,117 @@ proof(cases premise\<^sub>G conclusion\<^sub>G rule: ground.ground_eq_factoring.
     show  "select premise = {#}"
       using select_empty.
   next
-    have literal\<^sub>1_\<sigma>_in_premise: "literal\<^sub>1 \<cdot>l \<sigma> \<in># premise \<cdot> \<sigma>"
+    have literal\<^sub>1_\<mu>_in_premise: "literal\<^sub>1 \<cdot>l \<mu> \<in># premise \<cdot> \<mu>"
       using literal\<^sub>1_maximal(1) literal_in_clause_subst maximal\<^sub>l_in_clause by blast
 
-    have "is_maximal\<^sub>l (literal\<^sub>1 \<cdot>l \<sigma>) (premise \<cdot> \<sigma>)"
+    have "is_maximal\<^sub>l (literal\<^sub>1 \<cdot>l \<mu>) (premise \<cdot> \<mu>)"
       using is_maximal\<^sub>l_ground_subst_stability'[OF 
-          literal\<^sub>1_\<sigma>_in_premise 
-          premise_grounding[unfolded \<sigma>(2) clause_subst_compose]
-          literal\<^sub>1_maximal(2)[unfolded \<sigma>(2) clause_subst_compose literal_subst_compose]
+          literal\<^sub>1_\<mu>_in_premise 
+          premise_grounding[unfolded \<mu>(2) clause_subst_compose]
+          literal\<^sub>1_maximal(2)[unfolded \<mu>(2) clause_subst_compose literal_subst_compose]
           ].
 
-    then show "is_maximal\<^sub>l (literal\<^sub>1 \<cdot>l \<sigma>) (premise \<cdot> \<sigma>)"
+    then show "is_maximal\<^sub>l (literal\<^sub>1 \<cdot>l \<mu>) (premise \<cdot> \<mu>)"
       by blast
   next
-    have term_groundings: "is_ground_term (term\<^sub>1' \<cdot>t \<sigma> \<cdot>t \<tau>)" "is_ground_term (term\<^sub>1 \<cdot>t \<sigma> \<cdot>t \<tau>)" 
+    have term_groundings: "is_ground_term (term\<^sub>1' \<cdot>t \<mu> \<cdot>t \<sigma>)" "is_ground_term (term\<^sub>1 \<cdot>t \<mu> \<cdot>t \<sigma>)" 
       unfolding 
         term_subst_compose[symmetric] 
-        \<sigma>(2)[symmetric]
+        \<mu>(2)[symmetric]
         term\<^sub>G\<^sub>1_term\<^sub>1[symmetric] 
         term\<^sub>G\<^sub>2_term\<^sub>1'[symmetric] 
       using ground_term_is_ground
       by simp_all
 
-    have "term\<^sub>1' \<cdot>t \<sigma> \<cdot>t \<tau> \<prec>\<^sub>t term\<^sub>1 \<cdot>t \<sigma> \<cdot>t \<tau>"
+    have "term\<^sub>1' \<cdot>t \<mu> \<cdot>t \<sigma> \<prec>\<^sub>t term\<^sub>1 \<cdot>t \<mu> \<cdot>t \<sigma>"
       using ground_eq_factoringI(6)[unfolded 
           less\<^sub>t\<^sub>G_def 
           term\<^sub>G\<^sub>1_term\<^sub>1 
           term\<^sub>G\<^sub>2_term\<^sub>1'
-          \<sigma>(2) 
+          \<mu>(2) 
           term_subst_compose
           ].
 
-    then show "\<not> term\<^sub>1 \<cdot>t \<sigma> \<preceq>\<^sub>t term\<^sub>1' \<cdot>t \<sigma>"
+    then show "\<not> term\<^sub>1 \<cdot>t \<mu> \<preceq>\<^sub>t term\<^sub>1' \<cdot>t \<mu>"
       using less\<^sub>t_less_eq\<^sub>t_ground_subst_stability[OF term_groundings]
       by blast
   next 
-    show "term_subst.is_imgu \<sigma> {{term\<^sub>1, term\<^sub>2}}"
-      using \<sigma>(1).
+    show "term_subst.is_imgu \<mu> {{term\<^sub>1, term\<^sub>2}}"
+      using \<mu>(1).
   next 
-    show "?conclusion' \<cdot> \<sigma> = ?conclusion' \<cdot> \<sigma>"
+    show "?conclusion' \<cdot> \<mu> = ?conclusion' \<cdot> \<mu>"
       ..
   qed
 
-  have "term_subst.is_idem \<sigma>"
-    using \<sigma>(1)
+  have "term_subst.is_idem \<mu>"
+    using \<mu>(1)
     by (simp add: term_subst.is_imgu_iff_is_idem_and_is_mgu)  
 
-  then have \<sigma>_\<theta>: "\<sigma> \<odot> \<theta> = \<theta>"
-    unfolding \<sigma>(2) term_subst.is_idem_def
+  then have \<mu>_\<gamma>: "\<mu> \<odot> \<gamma> = \<gamma>"
+    unfolding \<mu>(2) term_subst.is_idem_def
     by (metis subst_compose_assoc)
 
-  have "conclusion \<cdot> \<theta> = 
+  have "conclusion \<cdot> \<gamma> = 
       add_mset (to_term term\<^sub>G\<^sub>2 !\<approx> to_term term\<^sub>G\<^sub>3) 
         (add_mset (to_term term\<^sub>G\<^sub>1 \<approx> to_term term\<^sub>G\<^sub>3) (to_clause premise'\<^sub>G))"
     using ground_eq_factoringI(7) to_ground_clause_inverse[OF conclusion_grounding]
     unfolding to_term_to_atom to_atom_to_literal to_clause_add_mset[symmetric]
     by simp
 
-  then have conclusion_\<theta>: 
-    "conclusion \<cdot> \<theta> = add_mset (term\<^sub>1 \<approx> term\<^sub>2') (add_mset (term\<^sub>1' !\<approx> term\<^sub>2') premise') \<cdot> \<theta>"
+  then have conclusion_\<gamma>: 
+    "conclusion \<cdot> \<gamma> = add_mset (term\<^sub>1 \<approx> term\<^sub>2') (add_mset (term\<^sub>1' !\<approx> term\<^sub>2') premise') \<cdot> \<gamma>"
     unfolding 
       term\<^sub>G\<^sub>2_term\<^sub>1'
       term\<^sub>G\<^sub>3_term\<^sub>2'
       term\<^sub>G\<^sub>1_term\<^sub>1
-      premise'_\<theta>[symmetric]
+      premise'_\<gamma>[symmetric]
       subst_clause_add_mset[symmetric]
       subst_literal[symmetric]
       subst_atom[symmetric]
     by (simp add: add_mset_commute)
 
-  then have "to_ground_clause (conclusion \<cdot> \<theta>) \<in> clause_groundings (?conclusion' \<cdot> \<sigma>)"
+  then have "to_ground_clause (conclusion \<cdot> \<gamma>) \<in> clause_groundings (?conclusion' \<cdot> \<mu>)"
     unfolding clause_groundings_def 
-    using \<sigma>(2) conclusion_\<theta> conclusion_grounding by auto
+    using \<mu>(2) conclusion_\<gamma> conclusion_grounding by auto
 
 (* TODO *)
   with eq_factoring that show ?thesis
     unfolding clause_groundings_def inference_groundings_def ground.G_Inf_def inferences_def 
     using premise_grounding
     apply auto
-    by (metis \<sigma>_\<theta> clause_subst_compose conclusion\<^sub>G conclusion_\<theta> conclusion_grounding ground_eq_factoring premise\<^sub>G)
+    by (metis \<mu>_\<gamma> clause_subst_compose conclusion\<^sub>G conclusion_\<gamma> conclusion_grounding ground_eq_factoring premise\<^sub>G)
 qed
 
 lemma superposition_lifting:
   fixes 
     premise\<^sub>G\<^sub>1 premise\<^sub>G\<^sub>2 conclusion\<^sub>G :: "'f gatom clause" and 
     premise\<^sub>1 premise\<^sub>2 conclusion :: "('f, 'v) atom clause" and
-    \<theta> \<rho>\<^sub>1 \<rho>\<^sub>2 :: "('f, 'v) subst"
+    \<gamma> \<rho>\<^sub>1 \<rho>\<^sub>2 :: "('f, 'v) subst"
   defines 
-    premise\<^sub>G\<^sub>1 [simp]: "premise\<^sub>G\<^sub>1 \<equiv> to_ground_clause (premise\<^sub>1 \<cdot> \<rho>\<^sub>1 \<cdot> \<theta>)" and
-    premise\<^sub>G\<^sub>2 [simp]: "premise\<^sub>G\<^sub>2 \<equiv> to_ground_clause (premise\<^sub>2 \<cdot> \<rho>\<^sub>2 \<cdot> \<theta>)" and
-    conclusion\<^sub>G [simp]: "conclusion\<^sub>G \<equiv> to_ground_clause (conclusion \<cdot> \<theta>)" and
+    premise\<^sub>G\<^sub>1 [simp]: "premise\<^sub>G\<^sub>1 \<equiv> to_ground_clause (premise\<^sub>1 \<cdot> \<rho>\<^sub>1 \<cdot> \<gamma>)" and
+    premise\<^sub>G\<^sub>2 [simp]: "premise\<^sub>G\<^sub>2 \<equiv> to_ground_clause (premise\<^sub>2 \<cdot> \<rho>\<^sub>2 \<cdot> \<gamma>)" and
+    conclusion\<^sub>G [simp]: "conclusion\<^sub>G \<equiv> to_ground_clause (conclusion \<cdot> \<gamma>)" and
     premise_groundings [simp]: 
-      "premise_groundings \<equiv> clause_groundings premise\<^sub>1 \<union> clause_groundings premise\<^sub>2" and
+    "premise_groundings \<equiv> clause_groundings premise\<^sub>1 \<union> clause_groundings premise\<^sub>2" and
     \<iota>\<^sub>G [simp]: "\<iota>\<^sub>G \<equiv> Infer [premise\<^sub>G\<^sub>2, premise\<^sub>G\<^sub>1] conclusion\<^sub>G"
   assumes 
     renaming: 
     "term_subst.is_renaming \<rho>\<^sub>1" 
     "term_subst.is_renaming \<rho>\<^sub>2" 
     "vars_clause (premise\<^sub>1 \<cdot> \<rho>\<^sub>1) \<inter> vars_clause (premise\<^sub>2 \<cdot> \<rho>\<^sub>2) = {}" and
-    premise\<^sub>1_grounding [intro]: "is_ground_clause (premise\<^sub>1 \<cdot> \<rho>\<^sub>1 \<cdot> \<theta>)" and
-    premise\<^sub>2_grounding [intro]: "is_ground_clause (premise\<^sub>2 \<cdot> \<rho>\<^sub>2 \<cdot> \<theta>)" and
-    conclusion_grounding [intro]: "is_ground_clause (conclusion \<cdot> \<theta>)" and
+    premise\<^sub>1_grounding [intro]: "is_ground_clause (premise\<^sub>1 \<cdot> \<rho>\<^sub>1 \<cdot> \<gamma>)" and
+    premise\<^sub>2_grounding [intro]: "is_ground_clause (premise\<^sub>2 \<cdot> \<rho>\<^sub>2 \<cdot> \<gamma>)" and
+    conclusion_grounding [intro]: "is_ground_clause (conclusion \<cdot> \<gamma>)" and
     select: 
-      "to_clause (select\<^sub>G premise\<^sub>G\<^sub>1) = (select premise\<^sub>1) \<cdot> \<rho>\<^sub>1 \<cdot> \<theta>"
-      "to_clause (select\<^sub>G premise\<^sub>G\<^sub>2) = (select premise\<^sub>2) \<cdot> \<rho>\<^sub>2 \<cdot> \<theta>" and
+    "to_clause (select\<^sub>G premise\<^sub>G\<^sub>1) = (select premise\<^sub>1) \<cdot> \<rho>\<^sub>1 \<cdot> \<gamma>"
+    "to_clause (select\<^sub>G premise\<^sub>G\<^sub>2) = (select premise\<^sub>2) \<cdot> \<rho>\<^sub>2 \<cdot> \<gamma>" and
     ground_superposition: "ground.ground_superposition premise\<^sub>G\<^sub>2 premise\<^sub>G\<^sub>1 conclusion\<^sub>G" and
     non_redundant: "\<iota>\<^sub>G \<notin> ground.Red_I premise_groundings"
   obtains conclusion' 
   where 
     "superposition premise\<^sub>2 premise\<^sub>1 conclusion'"
     "\<iota>\<^sub>G \<in> inference_groundings (Infer [premise\<^sub>2, premise\<^sub>1] conclusion')"
-    "conclusion' \<cdot> \<theta> = conclusion \<cdot> \<theta>"
+    "conclusion' \<cdot> \<gamma> = conclusion \<cdot> \<gamma>"
   using ground_superposition
 proof(cases premise\<^sub>G\<^sub>2 premise\<^sub>G\<^sub>1 conclusion\<^sub>G rule: ground.ground_superposition.cases)
   case (ground_superpositionI 
@@ -467,39 +470,39 @@ proof(cases premise\<^sub>G\<^sub>2 premise\<^sub>G\<^sub>1 conclusion\<^sub>G r
 
   have premise\<^sub>1_not_empty: "premise\<^sub>1 \<noteq> {#}"
     using ground_superpositionI(1) empty_not_add_mset clause_subst_empty premise\<^sub>G\<^sub>1
-    
+
     by (metis to_clause_empty_mset to_clause_inverse)
 
   have premise\<^sub>2_not_empty: "premise\<^sub>2 \<noteq> {#}"
     using ground_superpositionI(2) empty_not_add_mset clause_subst_empty premise\<^sub>G\<^sub>2
     by (metis to_clause_empty_mset to_clause_inverse)
 
-  have premise\<^sub>1_\<theta> : "premise\<^sub>1 \<cdot> \<rho>\<^sub>1 \<cdot> \<theta> = to_clause (add_mset literal\<^sub>G\<^sub>1 premise\<^sub>G\<^sub>1')"
+  have premise\<^sub>1_\<gamma> : "premise\<^sub>1 \<cdot> \<rho>\<^sub>1 \<cdot> \<gamma> = to_clause (add_mset literal\<^sub>G\<^sub>1 premise\<^sub>G\<^sub>1')"
     using ground_superpositionI(1) premise\<^sub>G\<^sub>1
     by (metis premise\<^sub>1_grounding to_ground_clause_inverse)
 
-  have premise\<^sub>2_\<theta> : "premise\<^sub>2 \<cdot> \<rho>\<^sub>2 \<cdot> \<theta> = to_clause (add_mset literal\<^sub>G\<^sub>2 premise\<^sub>G\<^sub>2')"
+  have premise\<^sub>2_\<gamma> : "premise\<^sub>2 \<cdot> \<rho>\<^sub>2 \<cdot> \<gamma> = to_clause (add_mset literal\<^sub>G\<^sub>2 premise\<^sub>G\<^sub>2')"
     using ground_superpositionI(2) premise\<^sub>G\<^sub>2
     by (metis premise\<^sub>2_grounding to_ground_clause_inverse)
 
-  let ?select\<^sub>G_empty = "select\<^sub>G (to_ground_clause (premise\<^sub>1 \<cdot> \<rho>\<^sub>1 \<cdot> \<theta>)) = {#}"
-  let ?select\<^sub>G_not_empty = "select\<^sub>G (to_ground_clause (premise\<^sub>1 \<cdot> \<rho>\<^sub>1 \<cdot> \<theta>)) \<noteq> {#}"
+  let ?select\<^sub>G_empty = "select\<^sub>G (to_ground_clause (premise\<^sub>1 \<cdot> \<rho>\<^sub>1 \<cdot> \<gamma>)) = {#}"
+  let ?select\<^sub>G_not_empty = "select\<^sub>G (to_ground_clause (premise\<^sub>1 \<cdot> \<rho>\<^sub>1 \<cdot> \<gamma>)) \<noteq> {#}"
 
   have pos_literal\<^sub>G\<^sub>1_is_strictly_maximal\<^sub>l: 
-    "\<P>\<^sub>G = Pos \<Longrightarrow> is_strictly_maximal\<^sub>l (to_literal literal\<^sub>G\<^sub>1) (premise\<^sub>1 \<cdot> \<rho>\<^sub>1 \<odot> \<theta>)"
+    "\<P>\<^sub>G = Pos \<Longrightarrow> is_strictly_maximal\<^sub>l (to_literal literal\<^sub>G\<^sub>1) (premise\<^sub>1 \<cdot> \<rho>\<^sub>1 \<odot> \<gamma>)"
     using ground_superpositionI(9)
     unfolding is_strictly_maximal\<^sub>G\<^sub>l_iff_is_strictly_maximal\<^sub>l
     by(simp add: premise\<^sub>1_grounding)
 
   have neg_literal\<^sub>G\<^sub>1_is_maximal\<^sub>l: 
-    "\<P>\<^sub>G = Neg \<Longrightarrow> ?select\<^sub>G_empty \<Longrightarrow> is_maximal\<^sub>l (to_literal literal\<^sub>G\<^sub>1) (premise\<^sub>1 \<cdot> \<rho>\<^sub>1 \<odot> \<theta>)"
+    "\<P>\<^sub>G = Neg \<Longrightarrow> ?select\<^sub>G_empty \<Longrightarrow> is_maximal\<^sub>l (to_literal literal\<^sub>G\<^sub>1) (premise\<^sub>1 \<cdot> \<rho>\<^sub>1 \<odot> \<gamma>)"
     using ground_superpositionI(9) premise\<^sub>G\<^sub>1
     unfolding is_maximal_lit_iff_is_maximal\<^sub>l 
-    by (metis clause_subst_compose diff_empty ground_superpositionI(1) id_remove_1_mset_iff_notin is_maximal\<^sub>l_if_is_strictly_maximal\<^sub>l is_maximal_lit_iff_is_maximal\<^sub>l maximal_lit_in_clause pos_literal\<^sub>G\<^sub>1_is_strictly_maximal\<^sub>l premise\<^sub>1_\<theta>)
+    by (metis clause_subst_compose diff_empty ground_superpositionI(1) id_remove_1_mset_iff_notin is_maximal\<^sub>l_if_is_strictly_maximal\<^sub>l is_maximal_lit_iff_is_maximal\<^sub>l maximal_lit_in_clause pos_literal\<^sub>G\<^sub>1_is_strictly_maximal\<^sub>l premise\<^sub>1_\<gamma>)
 
   obtain pos_literal\<^sub>1 where
     "is_strictly_maximal\<^sub>l pos_literal\<^sub>1 premise\<^sub>1"
-    "pos_literal\<^sub>1 \<cdot>l \<rho>\<^sub>1 \<odot> \<theta> = to_literal literal\<^sub>G\<^sub>1" 
+    "pos_literal\<^sub>1 \<cdot>l \<rho>\<^sub>1 \<odot> \<gamma> = to_literal literal\<^sub>G\<^sub>1" 
   if "\<P>\<^sub>G = Pos"
     using is_strictly_maximal\<^sub>l_ground_subst_stability[OF 
         premise\<^sub>1_grounding[folded clause_subst_compose] 
@@ -512,7 +515,7 @@ proof(cases premise\<^sub>G\<^sub>2 premise\<^sub>G\<^sub>1 conclusion\<^sub>G r
 
   moreover obtain neg_max_literal\<^sub>1 where
     "is_maximal\<^sub>l neg_max_literal\<^sub>1 premise\<^sub>1"
-    "neg_max_literal\<^sub>1 \<cdot>l \<rho>\<^sub>1 \<odot> \<theta> = to_literal literal\<^sub>G\<^sub>1" 
+    "neg_max_literal\<^sub>1 \<cdot>l \<rho>\<^sub>1 \<odot> \<gamma> = to_literal literal\<^sub>G\<^sub>1" 
   if "\<P>\<^sub>G = Neg" ?select\<^sub>G_empty
     using 
       is_maximal\<^sub>l_ground_subst_stability[OF 
@@ -527,7 +530,7 @@ proof(cases premise\<^sub>G\<^sub>2 premise\<^sub>G\<^sub>1 conclusion\<^sub>G r
 
   moreover obtain neg_selected_literal\<^sub>1 where
     "is_maximal\<^sub>l neg_selected_literal\<^sub>1 (select premise\<^sub>1)"
-    "neg_selected_literal\<^sub>1 \<cdot>l \<rho>\<^sub>1 \<odot> \<theta> = to_literal literal\<^sub>G\<^sub>1" 
+    "neg_selected_literal\<^sub>1 \<cdot>l \<rho>\<^sub>1 \<odot> \<gamma> = to_literal literal\<^sub>G\<^sub>1" 
   if "\<P>\<^sub>G = Neg" ?select\<^sub>G_not_empty 
     using ground_superpositionI(9) select(1) premise\<^sub>G\<^sub>1
     by (metis (no_types, opaque_lifting) clause_subst_compose clause_subst_empty(2) ground_clause_is_ground is_maximal\<^sub>l_ground_subst_stability is_maximal_lit_iff_is_maximal\<^sub>l to_clause_inverse to_ground_clause_empty_mset unique_maximal_in_ground_clause)
@@ -536,25 +539,25 @@ proof(cases premise\<^sub>G\<^sub>2 premise\<^sub>G\<^sub>1 conclusion\<^sub>G r
     by (meson maximal\<^sub>l_in_clause mset_subset_eqD select_subset)
 
   ultimately obtain literal\<^sub>1 where
-    literal\<^sub>1_\<theta>: "literal\<^sub>1 \<cdot>l \<rho>\<^sub>1 \<odot> \<theta> = to_literal literal\<^sub>G\<^sub>1" and
+    literal\<^sub>1_\<gamma>: "literal\<^sub>1 \<cdot>l \<rho>\<^sub>1 \<odot> \<gamma> = to_literal literal\<^sub>G\<^sub>1" and
     literal\<^sub>1_in_premise\<^sub>1: "literal\<^sub>1 \<in># premise\<^sub>1" and
     literal\<^sub>1_is_strictly_maximal: "\<P>\<^sub>G = Pos \<Longrightarrow> is_strictly_maximal\<^sub>l literal\<^sub>1 premise\<^sub>1" and
     literal\<^sub>1_is_maximal: "\<P>\<^sub>G = Neg \<Longrightarrow> ?select\<^sub>G_empty \<Longrightarrow> is_maximal\<^sub>l literal\<^sub>1 premise\<^sub>1" and
     literal\<^sub>1_selected: "\<P>\<^sub>G = Neg \<Longrightarrow> ?select\<^sub>G_not_empty \<Longrightarrow> is_maximal\<^sub>l literal\<^sub>1 (select premise\<^sub>1)"
     by (metis ground_superpositionI(9) literals_distinct(1))
 
-  then have literal\<^sub>1_grounding [intro]: "is_ground_literal (literal\<^sub>1 \<cdot>l \<rho>\<^sub>1 \<odot> \<theta>)"
+  then have literal\<^sub>1_grounding [intro]: "is_ground_literal (literal\<^sub>1 \<cdot>l \<rho>\<^sub>1 \<odot> \<gamma>)"
     by simp
 
   have literal\<^sub>G\<^sub>2_is_strictly_maximal\<^sub>l: 
-    "is_strictly_maximal\<^sub>l (to_literal literal\<^sub>G\<^sub>2) (premise\<^sub>2 \<cdot> \<rho>\<^sub>2 \<odot> \<theta>)"
+    "is_strictly_maximal\<^sub>l (to_literal literal\<^sub>G\<^sub>2) (premise\<^sub>2 \<cdot> \<rho>\<^sub>2 \<odot> \<gamma>)"
     using ground_superpositionI(11)
     unfolding is_strictly_maximal\<^sub>G\<^sub>l_iff_is_strictly_maximal\<^sub>l
     by (simp add: premise\<^sub>2_grounding)
 
   obtain literal\<^sub>2 where 
     literal\<^sub>2_maximal: "is_strictly_maximal\<^sub>l literal\<^sub>2 premise\<^sub>2" and
-    literal\<^sub>2_\<theta>: "literal\<^sub>2 \<cdot>l \<rho>\<^sub>2 \<odot> \<theta> = to_literal literal\<^sub>G\<^sub>2"
+    literal\<^sub>2_\<gamma>: "literal\<^sub>2 \<cdot>l \<rho>\<^sub>2 \<odot> \<gamma> = to_literal literal\<^sub>G\<^sub>2"
     using is_strictly_maximal\<^sub>l_ground_subst_stability[OF 
         premise\<^sub>2_grounding[folded clause_subst_compose] 
         literal\<^sub>G\<^sub>2_is_strictly_maximal\<^sub>l
@@ -563,29 +566,29 @@ proof(cases premise\<^sub>G\<^sub>2 premise\<^sub>G\<^sub>1 conclusion\<^sub>G r
   then have literal\<^sub>2_in_premise\<^sub>2: "literal\<^sub>2 \<in># premise\<^sub>2" 
     using strictly_maximal\<^sub>l_in_clause by blast
 
-  have literal\<^sub>2_grounding [intro]: "is_ground_literal (literal\<^sub>2 \<cdot>l \<rho>\<^sub>2 \<odot> \<theta>)"
-    using literal\<^sub>2_\<theta> by simp
+  have literal\<^sub>2_grounding [intro]: "is_ground_literal (literal\<^sub>2 \<cdot>l \<rho>\<^sub>2 \<odot> \<gamma>)"
+    using literal\<^sub>2_\<gamma> by simp
 
   obtain premise\<^sub>1' where premise\<^sub>1: "premise\<^sub>1 = add_mset literal\<^sub>1 premise\<^sub>1'"
     by (meson literal\<^sub>1_in_premise\<^sub>1 multi_member_split)
 
-  then have premise\<^sub>1'_\<theta>: "premise\<^sub>1' \<cdot> \<rho>\<^sub>1 \<cdot> \<theta> = to_clause premise\<^sub>G\<^sub>1'"
-    using premise\<^sub>1_\<theta>  
-    unfolding to_clause_add_mset literal\<^sub>1_\<theta>[symmetric]
+  then have premise\<^sub>1'_\<gamma>: "premise\<^sub>1' \<cdot> \<rho>\<^sub>1 \<cdot> \<gamma> = to_clause premise\<^sub>G\<^sub>1'"
+    using premise\<^sub>1_\<gamma>  
+    unfolding to_clause_add_mset literal\<^sub>1_\<gamma>[symmetric]
     by (simp add: subst_clause_add_mset)
 
   obtain premise\<^sub>2' where premise\<^sub>2: "premise\<^sub>2 = add_mset literal\<^sub>2 premise\<^sub>2'"
     by (meson literal\<^sub>2_in_premise\<^sub>2 multi_member_split)
 
-  then have premise\<^sub>2'_\<theta>: "premise\<^sub>2' \<cdot> \<rho>\<^sub>2 \<cdot> \<theta> = to_clause premise\<^sub>G\<^sub>2'"
-    using premise\<^sub>2_\<theta>  
-    unfolding to_clause_add_mset literal\<^sub>2_\<theta>[symmetric]
+  then have premise\<^sub>2'_\<gamma>: "premise\<^sub>2' \<cdot> \<rho>\<^sub>2 \<cdot> \<gamma> = to_clause premise\<^sub>G\<^sub>2'"
+    using premise\<^sub>2_\<gamma>  
+    unfolding to_clause_add_mset literal\<^sub>2_\<gamma>[symmetric]
     by (simp add: subst_clause_add_mset)
 
   let ?\<P> = "if \<P>\<^sub>G = Pos then Pos else Neg"
 
-  from literal\<^sub>1_\<theta> have literal\<^sub>1_\<theta>': 
-    "literal\<^sub>1 \<cdot>l \<rho>\<^sub>1 \<cdot>l \<theta> = ?\<P> (Upair (to_context context\<^sub>G)\<langle>to_term term\<^sub>G\<^sub>1\<rangle> (to_term term\<^sub>G\<^sub>2))"
+  from literal\<^sub>1_\<gamma> have literal\<^sub>1_\<gamma>': 
+    "literal\<^sub>1 \<cdot>l \<rho>\<^sub>1 \<cdot>l \<gamma> = ?\<P> (Upair (to_context context\<^sub>G)\<langle>to_term term\<^sub>G\<^sub>1\<rangle> (to_term term\<^sub>G\<^sub>2))"
     using ground_superpositionI(4)
     unfolding ground_superpositionI(5)
     by (cases "\<P>\<^sub>G = Pos") 
@@ -597,40 +600,40 @@ proof(cases premise\<^sub>G\<^sub>2 premise\<^sub>G\<^sub>1 conclusion\<^sub>G r
 
   then obtain term\<^sub>1_with_context term\<^sub>1' where 
     literal\<^sub>1: "literal\<^sub>1 = ?\<P> (Upair term\<^sub>1_with_context term\<^sub>1')" and
-    term\<^sub>1'_\<theta>: "term\<^sub>1' \<cdot>t \<rho>\<^sub>1 \<cdot>t \<theta> = to_term term\<^sub>G\<^sub>2" and
-    term\<^sub>1_with_context_\<theta>: "term\<^sub>1_with_context \<cdot>t \<rho>\<^sub>1 \<cdot>t \<theta> = (to_context context\<^sub>G)\<langle>to_term term\<^sub>G\<^sub>1\<rangle>"
+    term\<^sub>1'_\<gamma>: "term\<^sub>1' \<cdot>t \<rho>\<^sub>1 \<cdot>t \<gamma> = to_term term\<^sub>G\<^sub>2" and
+    term\<^sub>1_with_context_\<gamma>: "term\<^sub>1_with_context \<cdot>t \<rho>\<^sub>1 \<cdot>t \<gamma> = (to_context context\<^sub>G)\<langle>to_term term\<^sub>G\<^sub>1\<rangle>"
     by (smt (verit, ccfv_SIG) obtain_from_literal_subst)
 
-  have "to_ground_clause (premise\<^sub>1 \<cdot> \<rho>\<^sub>1 \<cdot> \<theta>) \<in> clause_groundings premise\<^sub>1"
+  have "to_ground_clause (premise\<^sub>1 \<cdot> \<rho>\<^sub>1 \<cdot> \<gamma>) \<in> clause_groundings premise\<^sub>1"
     unfolding clause_groundings_def
     by (smt (verit, del_insts) clause_subst_compose mem_Collect_eq premise\<^sub>1_grounding)
 
-  moreover have "to_ground_clause (premise\<^sub>2 \<cdot> \<rho>\<^sub>2 \<cdot> \<theta>) \<in> clause_groundings premise\<^sub>2"
+  moreover have "to_ground_clause (premise\<^sub>2 \<cdot> \<rho>\<^sub>2 \<cdot> \<gamma>) \<in> clause_groundings premise\<^sub>2"
     unfolding clause_groundings_def
     by (smt (verit, del_insts) clause_subst_compose mem_Collect_eq premise\<^sub>2_grounding)
 
-  moreover have conclusion_\<theta>\<^sub>G: "conclusion \<cdot> \<theta> = 
+  moreover have conclusion_\<gamma>\<^sub>G: "conclusion \<cdot> \<gamma> = 
     add_mset (?\<P> (Upair (to_context context\<^sub>G)\<langle>to_term term\<^sub>G\<^sub>3\<rangle> (to_term term\<^sub>G\<^sub>2))) 
       (to_clause premise\<^sub>G\<^sub>1' + to_clause premise\<^sub>G\<^sub>2')"
     using ground_superpositionI(4, 12) to_ground_clause_inverse[OF conclusion_grounding] 
     unfolding ground_term_with_context(3) to_term_to_atom
     by(cases "\<P>\<^sub>G = Pos")(simp_all add: to_atom_to_literal to_clause_add_mset)
 
-  from literal\<^sub>2_\<theta> have literal\<^sub>2_\<theta>': 
-    "literal\<^sub>2 \<cdot>l \<rho>\<^sub>2 \<cdot>l \<theta> = to_term term\<^sub>G\<^sub>1 \<approx> to_term term\<^sub>G\<^sub>3"
+  from literal\<^sub>2_\<gamma> have literal\<^sub>2_\<gamma>': 
+    "literal\<^sub>2 \<cdot>l \<rho>\<^sub>2 \<cdot>l \<gamma> = to_term term\<^sub>G\<^sub>1 \<approx> to_term term\<^sub>G\<^sub>3"
     unfolding ground_superpositionI(6) to_term_to_atom to_atom_to_literal(2) literal_subst_compose.
 
   then obtain term\<^sub>2 term\<^sub>2' where 
     literal\<^sub>2: "literal\<^sub>2 = term\<^sub>2 \<approx> term\<^sub>2'" and
-    term\<^sub>2_\<theta>: "term\<^sub>2 \<cdot>t \<rho>\<^sub>2 \<cdot>t \<theta> = to_term term\<^sub>G\<^sub>1" and     
-    term\<^sub>2'_\<theta>: "term\<^sub>2' \<cdot>t \<rho>\<^sub>2 \<cdot>t \<theta> = to_term term\<^sub>G\<^sub>3"
+    term\<^sub>2_\<gamma>: "term\<^sub>2 \<cdot>t \<rho>\<^sub>2 \<cdot>t \<gamma> = to_term term\<^sub>G\<^sub>1" and     
+    term\<^sub>2'_\<gamma>: "term\<^sub>2' \<cdot>t \<rho>\<^sub>2 \<cdot>t \<gamma> = to_term term\<^sub>G\<^sub>3"
     using obtain_from_pos_literal_subst
     by metis
 
   have special_case: "\<nexists>context\<^sub>1 term\<^sub>1. 
     term\<^sub>1_with_context = context\<^sub>1\<langle>term\<^sub>1\<rangle> \<and> 
-    term\<^sub>1 \<cdot>t \<rho>\<^sub>1 \<cdot>t \<theta> = to_term term\<^sub>G\<^sub>1 \<and> 
-    context\<^sub>1 \<cdot>t\<^sub>c \<rho>\<^sub>1 \<cdot>t\<^sub>c \<theta> = to_context context\<^sub>G \<and> 
+    term\<^sub>1 \<cdot>t \<rho>\<^sub>1 \<cdot>t \<gamma> = to_term term\<^sub>G\<^sub>1 \<and> 
+    context\<^sub>1 \<cdot>t\<^sub>c \<rho>\<^sub>1 \<cdot>t\<^sub>c \<gamma> = to_context context\<^sub>G \<and> 
     is_Fun term\<^sub>1 \<Longrightarrow>
       ground.redundant_infer
          (clause_groundings (add_mset literal\<^sub>1 premise\<^sub>1') \<union> clause_groundings (add_mset literal\<^sub>2 premise\<^sub>2'))
@@ -639,8 +642,8 @@ proof(cases premise\<^sub>G\<^sub>2 premise\<^sub>G\<^sub>1 conclusion\<^sub>G r
   proof-
     assume a: "\<nexists>context\<^sub>1 term\<^sub>1. 
       term\<^sub>1_with_context = context\<^sub>1\<langle>term\<^sub>1\<rangle> \<and> 
-      term\<^sub>1 \<cdot>t \<rho>\<^sub>1 \<cdot>t \<theta> = to_term term\<^sub>G\<^sub>1 \<and> 
-      context\<^sub>1 \<cdot>t\<^sub>c \<rho>\<^sub>1 \<cdot>t\<^sub>c \<theta> = to_context context\<^sub>G \<and> 
+      term\<^sub>1 \<cdot>t \<rho>\<^sub>1 \<cdot>t \<gamma> = to_term term\<^sub>G\<^sub>1 \<and> 
+      context\<^sub>1 \<cdot>t\<^sub>c \<rho>\<^sub>1 \<cdot>t\<^sub>c \<gamma> = to_context context\<^sub>G \<and> 
       is_Fun term\<^sub>1"
 
     have term\<^sub>1_with_context_not_ground: "\<not> is_ground_term term\<^sub>1_with_context"
@@ -649,19 +652,19 @@ proof(cases premise\<^sub>G\<^sub>2 premise\<^sub>G\<^sub>1 conclusion\<^sub>G r
 
       then obtain term\<^sub>1 context\<^sub>1 where
         "term\<^sub>1_with_context = context\<^sub>1\<langle>term\<^sub>1\<rangle>"
-        "term\<^sub>1 \<cdot>t \<rho>\<^sub>1 \<cdot>t \<theta> = to_term term\<^sub>G\<^sub>1" 
-        "context\<^sub>1 \<cdot>t\<^sub>c \<rho>\<^sub>1 \<cdot>t\<^sub>c \<theta> = to_context context\<^sub>G"
+        "term\<^sub>1 \<cdot>t \<rho>\<^sub>1 \<cdot>t \<gamma> = to_term term\<^sub>G\<^sub>1" 
+        "context\<^sub>1 \<cdot>t\<^sub>c \<rho>\<^sub>1 \<cdot>t\<^sub>c \<gamma> = to_context context\<^sub>G"
         "is_Fun term\<^sub>1"
-        by (metis ground_context_is_ground ground_term_is_ground subst_ground_context term\<^sub>1_with_context_\<theta> term_subst.subst_ident_if_ground gterm_is_fun)
+        by (metis ground_context_is_ground ground_term_is_ground subst_ground_context term\<^sub>1_with_context_\<gamma> term_subst.subst_ident_if_ground gterm_is_fun)
 
       with a show False
         by blast
     qed
 
-    with a term\<^sub>1_with_context_\<theta> have "\<exists>term\<^sub>x context\<^sub>x context\<^sub>x'. 
+    with a term\<^sub>1_with_context_\<gamma> have "\<exists>term\<^sub>x context\<^sub>x context\<^sub>x'. 
       term\<^sub>1_with_context = context\<^sub>x\<langle>term\<^sub>x\<rangle> \<and> 
       is_Var term\<^sub>x \<and> 
-      (context\<^sub>x \<cdot>t\<^sub>c \<rho>\<^sub>1 \<cdot>t\<^sub>c \<theta>) \<circ>\<^sub>c context\<^sub>x' = to_context context\<^sub>G"
+      (context\<^sub>x \<cdot>t\<^sub>c \<rho>\<^sub>1 \<cdot>t\<^sub>c \<gamma>) \<circ>\<^sub>c context\<^sub>x' = to_context context\<^sub>G"
     proof(induction term\<^sub>1_with_context arbitrary: context\<^sub>G)
       case (Var x)
       show ?case
@@ -677,18 +680,18 @@ proof(cases premise\<^sub>G\<^sub>2 premise\<^sub>G\<^sub>1 conclusion\<^sub>G r
         using Fun(3)
         by (smt (verit) ctxt_apply_term.simps(2) ctxt_of_gctxt.elims eval_term.simps(2) term.sel(2))
 
-      have xx: "map ((\<lambda>s. s \<cdot>t \<theta>) \<circ> (\<lambda>s. s \<cdot>t \<rho>\<^sub>1)) terms = map to_term ss1 @ (to_context context\<^sub>G')\<langle>to_term term\<^sub>G\<^sub>1\<rangle> # map to_term ss2"
+      have xx: "map ((\<lambda>s. s \<cdot>t \<gamma>) \<circ> (\<lambda>s. s \<cdot>t \<rho>\<^sub>1)) terms = map to_term ss1 @ (to_context context\<^sub>G')\<langle>to_term term\<^sub>G\<^sub>1\<rangle> # map to_term ss2"
         using Fun(3)
         unfolding context\<^sub>G
         by auto
 
       then obtain ts1 "term" ts2 where 
         terms: "terms = ts1 @ term # ts2" and
-        "map ((\<lambda>s. s \<cdot>t \<theta>) \<circ> (\<lambda>s. s \<cdot>t \<rho>\<^sub>1)) ts1 = map to_term ss1"
-        "map ((\<lambda>s. s \<cdot>t \<theta>) \<circ> (\<lambda>s. s \<cdot>t \<rho>\<^sub>1)) ts2 = map to_term ss2"
+        "map ((\<lambda>s. s \<cdot>t \<gamma>) \<circ> (\<lambda>s. s \<cdot>t \<rho>\<^sub>1)) ts1 = map to_term ss1"
+        "map ((\<lambda>s. s \<cdot>t \<gamma>) \<circ> (\<lambda>s. s \<cdot>t \<rho>\<^sub>1)) ts2 = map to_term ss2"
         by (smt (z3) append_eq_map_conv map_eq_Cons_conv)
 
-      with xx have yy: "term \<cdot>t \<rho>\<^sub>1 \<cdot>t \<theta> = (to_context context\<^sub>G')\<langle>to_term term\<^sub>G\<^sub>1\<rangle>"
+      with xx have yy: "term \<cdot>t \<rho>\<^sub>1 \<cdot>t \<gamma> = (to_context context\<^sub>G')\<langle>to_term term\<^sub>G\<^sub>1\<rangle>"
         by simp
 
       show ?case
@@ -696,18 +699,18 @@ proof(cases premise\<^sub>G\<^sub>2 premise\<^sub>G\<^sub>1 conclusion\<^sub>G r
         case True
         with yy obtain term\<^sub>1 context\<^sub>1 where zz: 
           "term = context\<^sub>1\<langle>term\<^sub>1\<rangle>"
-          "term\<^sub>1 \<cdot>t \<rho>\<^sub>1 \<cdot>t \<theta> = to_term term\<^sub>G\<^sub>1" "context\<^sub>1 \<cdot>t\<^sub>c \<rho>\<^sub>1 \<cdot>t\<^sub>c \<theta> = to_context context\<^sub>G'" "is_Fun term\<^sub>1"
+          "term\<^sub>1 \<cdot>t \<rho>\<^sub>1 \<cdot>t \<gamma> = to_term term\<^sub>G\<^sub>1" "context\<^sub>1 \<cdot>t\<^sub>c \<rho>\<^sub>1 \<cdot>t\<^sub>c \<gamma> = to_context context\<^sub>G'" "is_Fun term\<^sub>1"
           by (metis Term.ground_vars_term_empty ground_context_is_ground ground_subst_apply ground_term_is_ground subst_ground_context gterm_is_fun)
 
         then have zzz: "Fun f terms = (More f ts1 context\<^sub>1 ts2)\<langle>term\<^sub>1\<rangle>"
           unfolding terms
           by auto
 
-        have "\<exists>context\<^sub>1 term\<^sub>1. Fun f terms = context\<^sub>1\<langle>term\<^sub>1\<rangle> \<and> term\<^sub>1 \<cdot>t \<rho>\<^sub>1 \<cdot>t \<theta> = to_term term\<^sub>G\<^sub>1 \<and> context\<^sub>1 \<cdot>t\<^sub>c \<rho>\<^sub>1 \<cdot>t\<^sub>c \<theta> = to_context context\<^sub>G \<and> is_Fun term\<^sub>1"
+        have "\<exists>context\<^sub>1 term\<^sub>1. Fun f terms = context\<^sub>1\<langle>term\<^sub>1\<rangle> \<and> term\<^sub>1 \<cdot>t \<rho>\<^sub>1 \<cdot>t \<gamma> = to_term term\<^sub>G\<^sub>1 \<and> context\<^sub>1 \<cdot>t\<^sub>c \<rho>\<^sub>1 \<cdot>t\<^sub>c \<gamma> = to_context context\<^sub>G \<and> is_Fun term\<^sub>1"
           apply(rule exI[of _ "(More f ts1 context\<^sub>1 ts2)"])
           apply(rule exI[of _ term\<^sub>1])
           using zz zzz
-          by (auto simp add: \<open>map ((\<lambda>s. s \<cdot>t \<theta>) \<circ> (\<lambda>s. s \<cdot>t \<rho>\<^sub>1)) ts1 = map to_term ss1\<close> \<open>map ((\<lambda>s. s \<cdot>t \<theta>) \<circ> (\<lambda>s. s \<cdot>t \<rho>\<^sub>1)) ts2 = map to_term ss2\<close> context\<^sub>G)
+          by (auto simp add: \<open>map ((\<lambda>s. s \<cdot>t \<gamma>) \<circ> (\<lambda>s. s \<cdot>t \<rho>\<^sub>1)) ts1 = map to_term ss1\<close> \<open>map ((\<lambda>s. s \<cdot>t \<gamma>) \<circ> (\<lambda>s. s \<cdot>t \<rho>\<^sub>1)) ts2 = map to_term ss2\<close> context\<^sub>G)
 
         then show ?thesis
           using Fun(2)
@@ -717,14 +720,14 @@ proof(cases premise\<^sub>G\<^sub>2 premise\<^sub>G\<^sub>1 conclusion\<^sub>G r
         have zz: "term \<in> set terms"
           using terms by auto
 
-        have zzz: "\<nexists>context\<^sub>1 term\<^sub>1. term = context\<^sub>1\<langle>term\<^sub>1\<rangle> \<and> term\<^sub>1 \<cdot>t \<rho>\<^sub>1 \<cdot>t \<theta> = to_term term\<^sub>G\<^sub>1 \<and> context\<^sub>1 \<cdot>t\<^sub>c \<rho>\<^sub>1 \<cdot>t\<^sub>c \<theta> = to_context context\<^sub>G' \<and> is_Fun term\<^sub>1"
+        have zzz: "\<nexists>context\<^sub>1 term\<^sub>1. term = context\<^sub>1\<langle>term\<^sub>1\<rangle> \<and> term\<^sub>1 \<cdot>t \<rho>\<^sub>1 \<cdot>t \<gamma> = to_term term\<^sub>G\<^sub>1 \<and> context\<^sub>1 \<cdot>t\<^sub>c \<rho>\<^sub>1 \<cdot>t\<^sub>c \<gamma> = to_context context\<^sub>G' \<and> is_Fun term\<^sub>1"
         proof
-          assume "\<exists>context\<^sub>1 term\<^sub>1. term = context\<^sub>1\<langle>term\<^sub>1\<rangle> \<and> term\<^sub>1 \<cdot>t \<rho>\<^sub>1 \<cdot>t \<theta> = to_term term\<^sub>G\<^sub>1 \<and> context\<^sub>1 \<cdot>t\<^sub>c \<rho>\<^sub>1 \<cdot>t\<^sub>c \<theta> = to_context context\<^sub>G' \<and> is_Fun term\<^sub>1"
+          assume "\<exists>context\<^sub>1 term\<^sub>1. term = context\<^sub>1\<langle>term\<^sub>1\<rangle> \<and> term\<^sub>1 \<cdot>t \<rho>\<^sub>1 \<cdot>t \<gamma> = to_term term\<^sub>G\<^sub>1 \<and> context\<^sub>1 \<cdot>t\<^sub>c \<rho>\<^sub>1 \<cdot>t\<^sub>c \<gamma> = to_context context\<^sub>G' \<and> is_Fun term\<^sub>1"
 
           then obtain context\<^sub>1 term\<^sub>1 where
             "term": "term = context\<^sub>1\<langle>term\<^sub>1\<rangle>"
-            "term\<^sub>1 \<cdot>t \<rho>\<^sub>1 \<cdot>t \<theta> = to_term term\<^sub>G\<^sub>1"
-            "context\<^sub>1 \<cdot>t\<^sub>c \<rho>\<^sub>1 \<cdot>t\<^sub>c \<theta> = to_context context\<^sub>G'"
+            "term\<^sub>1 \<cdot>t \<rho>\<^sub>1 \<cdot>t \<gamma> = to_term term\<^sub>G\<^sub>1"
+            "context\<^sub>1 \<cdot>t\<^sub>c \<rho>\<^sub>1 \<cdot>t\<^sub>c \<gamma> = to_context context\<^sub>G'"
             "is_Fun term\<^sub>1"
             by blast
 
@@ -732,10 +735,10 @@ proof(cases premise\<^sub>G\<^sub>2 premise\<^sub>G\<^sub>1 conclusion\<^sub>G r
             unfolding terms
             by auto
 
-          have "\<exists>context\<^sub>1 term\<^sub>1. Fun f terms = context\<^sub>1\<langle>term\<^sub>1\<rangle> \<and> term\<^sub>1 \<cdot>t \<rho>\<^sub>1 \<cdot>t \<theta> = to_term term\<^sub>G\<^sub>1 \<and> context\<^sub>1 \<cdot>t\<^sub>c \<rho>\<^sub>1 \<cdot>t\<^sub>c \<theta> = to_context context\<^sub>G \<and> is_Fun term\<^sub>1"
+          have "\<exists>context\<^sub>1 term\<^sub>1. Fun f terms = context\<^sub>1\<langle>term\<^sub>1\<rangle> \<and> term\<^sub>1 \<cdot>t \<rho>\<^sub>1 \<cdot>t \<gamma> = to_term term\<^sub>G\<^sub>1 \<and> context\<^sub>1 \<cdot>t\<^sub>c \<rho>\<^sub>1 \<cdot>t\<^sub>c \<gamma> = to_context context\<^sub>G \<and> is_Fun term\<^sub>1"
             apply(rule exI[of _ "(More f ts1 context\<^sub>1 ts2)"])
             apply(rule exI[of _ term\<^sub>1])
-            by(auto simp: "term" terms \<open>map ((\<lambda>s. s \<cdot>t \<theta>) \<circ> (\<lambda>s. s \<cdot>t \<rho>\<^sub>1)) ts1 = map to_term ss1\<close> \<open>map ((\<lambda>s. s \<cdot>t \<theta>) \<circ> (\<lambda>s. s \<cdot>t \<rho>\<^sub>1)) ts2 = map to_term ss2\<close> context\<^sub>G)
+            by(auto simp: "term" terms \<open>map ((\<lambda>s. s \<cdot>t \<gamma>) \<circ> (\<lambda>s. s \<cdot>t \<rho>\<^sub>1)) ts1 = map to_term ss1\<close> \<open>map ((\<lambda>s. s \<cdot>t \<gamma>) \<circ> (\<lambda>s. s \<cdot>t \<rho>\<^sub>1)) ts2 = map to_term ss2\<close> context\<^sub>G)
 
 
           then show False
@@ -747,56 +750,56 @@ proof(cases premise\<^sub>G\<^sub>2 premise\<^sub>G\<^sub>1 conclusion\<^sub>G r
           term\<^sub>x: 
           "term = context\<^sub>x\<langle>term\<^sub>x\<rangle>"  
           "is_Var term\<^sub>x" 
-          "(context\<^sub>x \<cdot>t\<^sub>c \<rho>\<^sub>1 \<cdot>t\<^sub>c \<theta>) \<circ>\<^sub>c context\<^sub>x' = to_context context\<^sub>G'"
+          "(context\<^sub>x \<cdot>t\<^sub>c \<rho>\<^sub>1 \<cdot>t\<^sub>c \<gamma>) \<circ>\<^sub>c context\<^sub>x' = to_context context\<^sub>G'"
           using Fun(1)[OF zz zzz yy False] by blast
 
         show ?thesis
           apply(rule exI[of _ term\<^sub>x]) 
           apply(rule exI[of _ "(More f ts1 context\<^sub>x ts2)"])
           apply(rule exI[of _ context\<^sub>x'])
-          by(auto simp: term\<^sub>x terms \<open>map ((\<lambda>s. s \<cdot>t \<theta>) \<circ> (\<lambda>s. s \<cdot>t \<rho>\<^sub>1)) ts1 = map to_term ss1\<close> \<open>map ((\<lambda>s. s \<cdot>t \<theta>) \<circ> (\<lambda>s. s \<cdot>t \<rho>\<^sub>1)) ts2 = map to_term ss2\<close> context\<^sub>G)
+          by(auto simp: term\<^sub>x terms \<open>map ((\<lambda>s. s \<cdot>t \<gamma>) \<circ> (\<lambda>s. s \<cdot>t \<rho>\<^sub>1)) ts1 = map to_term ss1\<close> \<open>map ((\<lambda>s. s \<cdot>t \<gamma>) \<circ> (\<lambda>s. s \<cdot>t \<rho>\<^sub>1)) ts2 = map to_term ss2\<close> context\<^sub>G)
       qed
     qed
 
     then obtain term\<^sub>x context\<^sub>x context\<^sub>x' where
       context\<^sub>x: "term\<^sub>1_with_context = context\<^sub>x\<langle>term\<^sub>x\<rangle>"
       "is_Var term\<^sub>x"
-      "(context\<^sub>x \<circ>\<^sub>c context\<^sub>x') \<cdot>t\<^sub>c \<rho>\<^sub>1 \<cdot>t\<^sub>c \<theta> = to_context context\<^sub>G"
+      "(context\<^sub>x \<circ>\<^sub>c context\<^sub>x') \<cdot>t\<^sub>c \<rho>\<^sub>1 \<cdot>t\<^sub>c \<gamma> = to_context context\<^sub>G"
       by (metis Subterm_and_Context.ctxt_ctxt_compose ground_context_is_ground ground_term_is_ground ground_term_with_context_is_ground2(2) subst_compose_ctxt_compose_distrib subst_ground_context sup_bot.right_neutral vars_term_ctxt_apply)
 
     then obtain var\<^sub>x where var\<^sub>x: "Var var\<^sub>x = term\<^sub>x \<cdot>t \<rho>\<^sub>1"
       by (metis eval_term.simps(1) is_Var_def renaming(1) subst_cannot_add_var subst_compose_def term_subst.is_renaming_def)
 
-    obtain \<theta>' where \<theta>':
-      "\<theta>' = \<theta>(var\<^sub>x := (context\<^sub>x' \<cdot>t\<^sub>c \<rho>\<^sub>1 \<cdot>t\<^sub>c \<theta>)\<langle>to_term term\<^sub>G\<^sub>3\<rangle>)"
+    obtain \<gamma>' where \<gamma>':
+      "\<gamma>' = \<gamma>(var\<^sub>x := (context\<^sub>x' \<cdot>t\<^sub>c \<rho>\<^sub>1 \<cdot>t\<^sub>c \<gamma>)\<langle>to_term term\<^sub>G\<^sub>3\<rangle>)"
       by simp
 
-    have update_grounding: "is_ground_term (context\<^sub>x' \<cdot>t\<^sub>c \<rho>\<^sub>1 \<cdot>t\<^sub>c \<theta>)\<langle>to_term term\<^sub>G\<^sub>3\<rangle>"
+    have update_grounding: "is_ground_term (context\<^sub>x' \<cdot>t\<^sub>c \<rho>\<^sub>1 \<cdot>t\<^sub>c \<gamma>)\<langle>to_term term\<^sub>G\<^sub>3\<rangle>"
       by (metis Subterm_and_Context.ctxt_ctxt_compose context\<^sub>x(3) ground_term_with_context_is_ground1 ground_term_with_context_is_ground2(2) subst_compose_ctxt_compose_distrib)
 
-    have premise\<^sub>1_grounding': "is_ground_clause (add_mset literal\<^sub>1 premise\<^sub>1' \<cdot> \<rho>\<^sub>1 \<cdot> \<theta>)"
+    have premise\<^sub>1_grounding': "is_ground_clause (add_mset literal\<^sub>1 premise\<^sub>1' \<cdot> \<rho>\<^sub>1 \<cdot> \<gamma>)"
       using premise\<^sub>1 premise\<^sub>1_grounding by blast
 
-    have \<theta>'_grounding: "is_ground_clause (add_mset literal\<^sub>1 premise\<^sub>1' \<cdot> \<rho>\<^sub>1 \<cdot> \<theta>')"
+    have \<gamma>'_grounding: "is_ground_clause (add_mset literal\<^sub>1 premise\<^sub>1' \<cdot> \<rho>\<^sub>1 \<cdot> \<gamma>')"
       using ground_clause_subst_upd[OF update_grounding premise\<^sub>1_grounding']
-      unfolding \<theta>'
+      unfolding \<gamma>'
       by blast
 
-    let ?D = "to_ground_clause ((add_mset literal\<^sub>1 premise\<^sub>1') \<cdot> \<rho>\<^sub>1 \<cdot> \<theta>')"
+    let ?D = "to_ground_clause ((add_mset literal\<^sub>1 premise\<^sub>1') \<cdot> \<rho>\<^sub>1 \<cdot> \<gamma>')"
     let ?DD = "{ ?D }"
 
-    have term\<^sub>x_\<theta>: "to_ground_term (term\<^sub>x \<cdot>t \<rho>\<^sub>1 \<cdot>t \<theta>) = (to_ground_context (context\<^sub>x' \<cdot>t\<^sub>c \<rho>\<^sub>1 \<cdot>t\<^sub>c \<theta>))\<langle>term\<^sub>G\<^sub>1\<rangle>\<^sub>G"
-      using term\<^sub>1_with_context_\<theta>
+    have term\<^sub>x_\<gamma>: "to_ground_term (term\<^sub>x \<cdot>t \<rho>\<^sub>1 \<cdot>t \<gamma>) = (to_ground_context (context\<^sub>x' \<cdot>t\<^sub>c \<rho>\<^sub>1 \<cdot>t\<^sub>c \<gamma>))\<langle>term\<^sub>G\<^sub>1\<rangle>\<^sub>G"
+      using term\<^sub>1_with_context_\<gamma>
       unfolding context\<^sub>x(1)context\<^sub>x(3)[symmetric]
       apply auto
       by (metis ground_term_is_ground ground_term_with_context1 ground_term_with_context_is_ground2(1) update_grounding to_term_inverse)
 
-    have term\<^sub>x_\<theta>': "to_ground_term (term\<^sub>x \<cdot>t \<rho>\<^sub>1 \<cdot>t \<theta>') = (to_ground_context (context\<^sub>x' \<cdot>t\<^sub>c \<rho>\<^sub>1 \<cdot>t\<^sub>c \<theta>))\<langle>term\<^sub>G\<^sub>3\<rangle>\<^sub>G"
-      unfolding \<theta>'
+    have term\<^sub>x_\<gamma>': "to_ground_term (term\<^sub>x \<cdot>t \<rho>\<^sub>1 \<cdot>t \<gamma>') = (to_ground_context (context\<^sub>x' \<cdot>t\<^sub>c \<rho>\<^sub>1 \<cdot>t\<^sub>c \<gamma>))\<langle>term\<^sub>G\<^sub>3\<rangle>\<^sub>G"
+      unfolding \<gamma>'
       by (metis eval_term.simps(1) fun_upd_same ground_term_is_ground ground_term_with_context1 ground_term_with_context_is_ground2(1) update_grounding to_term_inverse var\<^sub>x)
 
-    have premise\<^sub>1_\<theta>_x: "add_mset literal\<^sub>1 premise\<^sub>1' \<cdot> \<rho>\<^sub>1 \<cdot> \<theta> =  add_mset (to_literal literal\<^sub>G\<^sub>1) (to_clause premise\<^sub>G\<^sub>1')"
-      using premise\<^sub>1 premise\<^sub>1_\<theta> to_clause_add_mset by auto
+    have premise\<^sub>1_\<gamma>_x: "add_mset literal\<^sub>1 premise\<^sub>1' \<cdot> \<rho>\<^sub>1 \<cdot> \<gamma> =  add_mset (to_literal literal\<^sub>G\<^sub>1) (to_clause premise\<^sub>G\<^sub>1')"
+      using premise\<^sub>1 premise\<^sub>1_\<gamma> to_clause_add_mset by auto
 
     have entails: "\<And>I. refl I \<Longrightarrow>
          trans I \<Longrightarrow>
@@ -815,8 +818,8 @@ proof(cases premise\<^sub>G\<^sub>2 premise\<^sub>G\<^sub>1 conclusion\<^sub>G r
         compatible_with_gctxt: "compatible_with_gctxt I" and
         premise: "?I \<TTurnstile>s {add_mset literal\<^sub>G\<^sub>2 premise\<^sub>G\<^sub>2', ?D}"
 
-      have var\<^sub>x_\<theta>_ground: "is_ground_term (Var var\<^sub>x \<cdot>t \<theta>)"
-        by (metis context\<^sub>x(1) ground_term_is_ground ground_term_with_context3 ground_term_with_context_is_ground2(2) subst_apply_term_ctxt_apply_distrib term\<^sub>1_with_context_\<theta> var\<^sub>x)
+      have var\<^sub>x_\<gamma>_ground: "is_ground_term (Var var\<^sub>x \<cdot>t \<gamma>)"
+        by (metis context\<^sub>x(1) ground_term_is_ground ground_term_with_context3 ground_term_with_context_is_ground2(2) subst_apply_term_ctxt_apply_distrib term\<^sub>1_with_context_\<gamma> var\<^sub>x)
 
       show "?I \<TTurnstile>s {add_mset (\<P>\<^sub>G (Upair context\<^sub>G\<langle>term\<^sub>G\<^sub>3\<rangle>\<^sub>G term\<^sub>G\<^sub>2)) (premise\<^sub>G\<^sub>1' + premise\<^sub>G\<^sub>2')}"
       proof(cases "?I \<TTurnstile> premise\<^sub>G\<^sub>2'")
@@ -824,7 +827,7 @@ proof(cases premise\<^sub>G\<^sub>2 premise\<^sub>G\<^sub>1 conclusion\<^sub>G r
         then show ?thesis 
           by auto
       next
-        let ?x =  "to_ground_context (context\<^sub>x' \<cdot>t\<^sub>c \<rho>\<^sub>1 \<cdot>t\<^sub>c \<theta>)"
+        let ?x =  "to_ground_context (context\<^sub>x' \<cdot>t\<^sub>c \<rho>\<^sub>1 \<cdot>t\<^sub>c \<gamma>)"
         case False
         then have literal\<^sub>G\<^sub>2: "?I \<TTurnstile>l literal\<^sub>G\<^sub>2"
           using premise by blast
@@ -833,18 +836,18 @@ proof(cases premise\<^sub>G\<^sub>2 premise\<^sub>G\<^sub>1 conclusion\<^sub>G r
           unfolding ground_superpositionI(6)
           using compatible_with_gctxt compatible_with_gctxt_def sym by auto
 
-        then have "?I \<TTurnstile>l to_ground_term (term\<^sub>x \<cdot>t \<rho>\<^sub>1 \<cdot>t \<theta>) \<approx> to_ground_term (term\<^sub>x \<cdot>t \<rho>\<^sub>1 \<cdot>t \<theta>')"
-          using term\<^sub>x_\<theta> term\<^sub>x_\<theta>'
+        then have "?I \<TTurnstile>l to_ground_term (term\<^sub>x \<cdot>t \<rho>\<^sub>1 \<cdot>t \<gamma>) \<approx> to_ground_term (term\<^sub>x \<cdot>t \<rho>\<^sub>1 \<cdot>t \<gamma>')"
+          using term\<^sub>x_\<gamma> term\<^sub>x_\<gamma>'
           by argo
 
-        then have "?I \<TTurnstile> to_ground_clause (add_mset literal\<^sub>1 premise\<^sub>1' \<cdot> \<rho>\<^sub>1 \<cdot> \<theta>')"
+        then have "?I \<TTurnstile> to_ground_clause (add_mset literal\<^sub>1 premise\<^sub>1' \<cdot> \<rho>\<^sub>1 \<cdot> \<gamma>')"
           using premise by fastforce
 
-        then have "?I \<TTurnstile> to_ground_clause (add_mset literal\<^sub>1 premise\<^sub>1' \<cdot> \<rho>\<^sub>1 \<cdot> \<theta>)"
-          using \<theta>'_grounding
-          unfolding \<theta>'
-          using interpretation_clause_congruence[OF trans sym compatible_with_gctxt update_grounding var\<^sub>x_\<theta>_ground]
-          using \<open>(\<lambda>(x, y). Upair x y) ` I \<TTurnstile>l to_ground_term (term\<^sub>x \<cdot>t \<rho>\<^sub>1 \<cdot>t \<theta>) \<approx> to_ground_term (term\<^sub>x \<cdot>t \<rho>\<^sub>1 \<cdot>t \<theta>')\<close> \<theta>' premise\<^sub>1_grounding' var\<^sub>x by auto
+        then have "?I \<TTurnstile> to_ground_clause (add_mset literal\<^sub>1 premise\<^sub>1' \<cdot> \<rho>\<^sub>1 \<cdot> \<gamma>)"
+          using \<gamma>'_grounding
+          unfolding \<gamma>'
+          using interpretation_clause_congruence[OF trans sym compatible_with_gctxt update_grounding var\<^sub>x_\<gamma>_ground]
+          using \<open>(\<lambda>(x, y). Upair x y) ` I \<TTurnstile>l to_ground_term (term\<^sub>x \<cdot>t \<rho>\<^sub>1 \<cdot>t \<gamma>) \<approx> to_ground_term (term\<^sub>x \<cdot>t \<rho>\<^sub>1 \<cdot>t \<gamma>')\<close> \<gamma>' premise\<^sub>1_grounding' var\<^sub>x by auto
 
         then have "?I \<TTurnstile> add_mset (\<P>\<^sub>G (Upair context\<^sub>G\<langle>term\<^sub>G\<^sub>1\<rangle>\<^sub>G term\<^sub>G\<^sub>2)) premise\<^sub>G\<^sub>1'"
           using ground_superpositionI(1) ground_superpositionI(5) premise\<^sub>1 by auto
@@ -865,50 +868,50 @@ proof(cases premise\<^sub>G\<^sub>2 premise\<^sub>G\<^sub>1 conclusion\<^sub>G r
 
     qed
 
-    have var\<^sub>x_\<theta>: "\<theta> var\<^sub>x = term\<^sub>x \<cdot>t \<rho>\<^sub>1 \<cdot>t \<theta>"
+    have var\<^sub>x_\<gamma>: "\<gamma> var\<^sub>x = term\<^sub>x \<cdot>t \<rho>\<^sub>1 \<cdot>t \<gamma>"
       using var\<^sub>x
       by simp
 
-    have smaller': "((context\<^sub>x \<circ>\<^sub>c context\<^sub>x') \<cdot>t\<^sub>c \<rho>\<^sub>1 \<cdot>t\<^sub>c \<theta>)\<langle>to_term term\<^sub>G\<^sub>3\<rangle> \<prec>\<^sub>t context\<^sub>x\<langle>term\<^sub>x\<rangle> \<cdot>t \<rho>\<^sub>1 \<cdot>t \<theta>"
+    have smaller': "((context\<^sub>x \<circ>\<^sub>c context\<^sub>x') \<cdot>t\<^sub>c \<rho>\<^sub>1 \<cdot>t\<^sub>c \<gamma>)\<langle>to_term term\<^sub>G\<^sub>3\<rangle> \<prec>\<^sub>t context\<^sub>x\<langle>term\<^sub>x\<rangle> \<cdot>t \<rho>\<^sub>1 \<cdot>t \<gamma>"
       unfolding context\<^sub>x(3) context\<^sub>x(1)[symmetric]
-      unfolding term\<^sub>1_with_context_\<theta>
+      unfolding term\<^sub>1_with_context_\<gamma>
       by (simp add: ground_superpositionI(8) less\<^sub>t_less\<^sub>t\<^sub>G)
 
-    then have xx: "(context\<^sub>x' \<cdot>t\<^sub>c \<rho>\<^sub>1 \<cdot>t\<^sub>c \<theta>)\<langle>to_term term\<^sub>G\<^sub>3\<rangle> \<prec>\<^sub>t \<theta> var\<^sub>x"
-      unfolding var\<^sub>x_\<theta>
-      using less\<^sub>t_ground_context_compatible'[of "context\<^sub>x \<cdot>t\<^sub>c \<rho>\<^sub>1 \<cdot>t\<^sub>c \<theta>" "(context\<^sub>x' \<cdot>t\<^sub>c \<rho>\<^sub>1 \<cdot>t\<^sub>c \<theta>)\<langle>to_term term\<^sub>G\<^sub>3\<rangle>" "term\<^sub>x \<cdot>t \<rho>\<^sub>1 \<cdot>t \<theta>"]
-      by (metis Subterm_and_Context.ctxt_ctxt_compose context\<^sub>x(1) ground_term_with_context_is_ground1 ground_term_with_context_is_ground2(1) ground_term_with_context_is_ground2(2) update_grounding subst_compose_ctxt_compose_distrib term\<^sub>1_with_context_\<theta> subst_apply_term_ctxt_apply_distrib)
+    then have xx: "(context\<^sub>x' \<cdot>t\<^sub>c \<rho>\<^sub>1 \<cdot>t\<^sub>c \<gamma>)\<langle>to_term term\<^sub>G\<^sub>3\<rangle> \<prec>\<^sub>t \<gamma> var\<^sub>x"
+      unfolding var\<^sub>x_\<gamma>
+      using less\<^sub>t_ground_context_compatible'[of "context\<^sub>x \<cdot>t\<^sub>c \<rho>\<^sub>1 \<cdot>t\<^sub>c \<gamma>" "(context\<^sub>x' \<cdot>t\<^sub>c \<rho>\<^sub>1 \<cdot>t\<^sub>c \<gamma>)\<langle>to_term term\<^sub>G\<^sub>3\<rangle>" "term\<^sub>x \<cdot>t \<rho>\<^sub>1 \<cdot>t \<gamma>"]
+      by (metis Subterm_and_Context.ctxt_ctxt_compose context\<^sub>x(1) ground_term_with_context_is_ground1 ground_term_with_context_is_ground2(1) ground_term_with_context_is_ground2(2) update_grounding subst_compose_ctxt_compose_distrib term\<^sub>1_with_context_\<gamma> subst_apply_term_ctxt_apply_distrib)
 
     have xy: "var\<^sub>x \<in> vars_literal (literal\<^sub>1  \<cdot>l \<rho>\<^sub>1)"
       unfolding literal\<^sub>1 context\<^sub>x vars_literal_def vars_atom_def 
       using var\<^sub>x
       by(auto simp: subst_literal subst_atom)
 
-    have "is_ground_literal (literal\<^sub>1 \<cdot>l \<rho>\<^sub>1 \<cdot>l \<theta>)"
+    have "is_ground_literal (literal\<^sub>1 \<cdot>l \<rho>\<^sub>1 \<cdot>l \<gamma>)"
       using literal\<^sub>1_grounding by force
 
-    then have smaller: "literal\<^sub>1 \<cdot>l \<rho>\<^sub>1 \<cdot>l \<theta>' \<prec>\<^sub>l literal\<^sub>1 \<cdot>l \<rho>\<^sub>1 \<cdot>l \<theta>"
-      unfolding \<theta>'
-      using less\<^sub>l_subst_upd[of _ \<theta>, OF update_grounding xx _ xy]
+    then have smaller: "literal\<^sub>1 \<cdot>l \<rho>\<^sub>1 \<cdot>l \<gamma>' \<prec>\<^sub>l literal\<^sub>1 \<cdot>l \<rho>\<^sub>1 \<cdot>l \<gamma>"
+      unfolding \<gamma>'
+      using less\<^sub>l_subst_upd[of _ \<gamma>, OF update_grounding xx _ xy]
       by blast
 
-    have premise\<^sub>1'_\<theta>_grounding: "is_ground_clause (premise\<^sub>1' \<cdot> \<rho>\<^sub>1 \<cdot> \<theta>)"
-      using premise\<^sub>1'_\<theta>
+    have premise\<^sub>1'_\<gamma>_grounding: "is_ground_clause (premise\<^sub>1' \<cdot> \<rho>\<^sub>1 \<cdot> \<gamma>)"
+      using premise\<^sub>1'_\<gamma>
       by simp
 
-    have smaller_premise\<^sub>1': "premise\<^sub>1' \<cdot> \<rho>\<^sub>1 \<cdot> \<theta>' \<preceq>\<^sub>c premise\<^sub>1' \<cdot> \<rho>\<^sub>1 \<cdot> \<theta>"
-      unfolding \<theta>'
+    have smaller_premise\<^sub>1': "premise\<^sub>1' \<cdot> \<rho>\<^sub>1 \<cdot> \<gamma>' \<preceq>\<^sub>c premise\<^sub>1' \<cdot> \<rho>\<^sub>1 \<cdot> \<gamma>"
+      unfolding \<gamma>'
       using 
-        less\<^sub>c_subst_upd[of _ \<theta>, OF update_grounding xx premise\<^sub>1'_\<theta>_grounding]
+        less\<^sub>c_subst_upd[of _ \<gamma>, OF update_grounding xx premise\<^sub>1'_\<gamma>_grounding]
       by (metis (no_types, lifting) clause_subst_eq fun_upd_other reflclp_iff)
 
-    from \<theta>'_grounding have "?D \<in> clause_groundings (add_mset literal\<^sub>1 premise\<^sub>1')"
+    from \<gamma>'_grounding have "?D \<in> clause_groundings (add_mset literal\<^sub>1 premise\<^sub>1')"
       unfolding clause_groundings_def clause_subst_compose[symmetric]
       by blast
 
     moreover have "?D \<prec>\<^sub>c\<^sub>G add_mset literal\<^sub>G\<^sub>1 premise\<^sub>G\<^sub>1'"
-      unfolding less\<^sub>c\<^sub>G_less\<^sub>c to_ground_clause_inverse[OF \<theta>'_grounding] to_clause_add_mset
-      unfolding literal\<^sub>1_\<theta>[symmetric]  subst_clause_add_mset premise\<^sub>1'_\<theta>[symmetric]
+      unfolding less\<^sub>c\<^sub>G_less\<^sub>c to_ground_clause_inverse[OF \<gamma>'_grounding] to_clause_add_mset
+      unfolding literal\<^sub>1_\<gamma>[symmetric]  subst_clause_add_mset premise\<^sub>1'_\<gamma>[symmetric]
       using less\<^sub>c_add_mset[OF smaller smaller_premise\<^sub>1']
       by simp
 
@@ -936,65 +939,65 @@ proof(cases premise\<^sub>G\<^sub>2 premise\<^sub>G\<^sub>1 conclusion\<^sub>G r
          (Infer [add_mset literal\<^sub>G\<^sub>2 premise\<^sub>G\<^sub>2', add_mset literal\<^sub>G\<^sub>1 premise\<^sub>G\<^sub>1']
            (to_ground_clause
              (add_mset ((if \<P>\<^sub>G = Pos then Pos else Neg) (Upair (to_context context\<^sub>G)\<langle>to_term term\<^sub>G\<^sub>3\<rangle> (to_term term\<^sub>G\<^sub>2))) (to_clause premise\<^sub>G\<^sub>1' + to_clause premise\<^sub>G\<^sub>2'))))\<rbrakk>
-    \<Longrightarrow> \<exists>context\<^sub>1 term\<^sub>1. term\<^sub>1_with_context = context\<^sub>1\<langle>term\<^sub>1\<rangle> \<and> context\<^sub>1 \<cdot>t\<^sub>c \<rho>\<^sub>1 \<cdot>t\<^sub>c \<theta> = to_context context\<^sub>G \<and> term\<^sub>1 \<cdot>t \<rho>\<^sub>1 \<cdot>t \<theta> = to_term term\<^sub>G\<^sub>1 \<and> is_Fun term\<^sub>1"
+    \<Longrightarrow> \<exists>context\<^sub>1 term\<^sub>1. term\<^sub>1_with_context = context\<^sub>1\<langle>term\<^sub>1\<rangle> \<and> context\<^sub>1 \<cdot>t\<^sub>c \<rho>\<^sub>1 \<cdot>t\<^sub>c \<gamma> = to_context context\<^sub>G \<and> term\<^sub>1 \<cdot>t \<rho>\<^sub>1 \<cdot>t \<gamma> = to_term term\<^sub>G\<^sub>1 \<and> is_Fun term\<^sub>1"
     unfolding z
     using special_case
     by blast
 
   obtain context\<^sub>1 term\<^sub>1 where 
     term\<^sub>1_with_context: "term\<^sub>1_with_context = context\<^sub>1\<langle>term\<^sub>1\<rangle>" and
-    term\<^sub>1_\<theta> : "term\<^sub>1 \<cdot>t \<rho>\<^sub>1 \<cdot>t \<theta> = to_term term\<^sub>G\<^sub>1" and
-    context\<^sub>1_\<theta> : "context\<^sub>1 \<cdot>t\<^sub>c \<rho>\<^sub>1 \<cdot>t\<^sub>c \<theta> = to_context context\<^sub>G" and
+    term\<^sub>1_\<gamma> : "term\<^sub>1 \<cdot>t \<rho>\<^sub>1 \<cdot>t \<gamma> = to_term term\<^sub>G\<^sub>1" and
+    context\<^sub>1_\<gamma> : "context\<^sub>1 \<cdot>t\<^sub>c \<rho>\<^sub>1 \<cdot>t\<^sub>c \<gamma> = to_context context\<^sub>G" and
     term\<^sub>1_not_Var: "\<not> is_Var term\<^sub>1"
     using non_redundant ground_superposition
-    unfolding premise\<^sub>1_\<theta>
-    unfolding premise\<^sub>2_\<theta>
-    unfolding conclusion_\<theta>\<^sub>G
+    unfolding premise\<^sub>1_\<gamma>
+    unfolding premise\<^sub>2_\<gamma>
+    unfolding conclusion_\<gamma>\<^sub>G
     unfolding premise\<^sub>1 premise\<^sub>2
     apply auto
     unfolding ground.Red_I_def
     apply auto
     unfolding ground.G_Inf_def
-     apply blast
-    by (metis conclusion\<^sub>G ground_superpositionI(12) premise\<^sub>1 premise\<^sub>1_\<theta> premise\<^sub>2 premise\<^sub>2_\<theta> special_case to_clause_inverse)
+    apply blast
+    by (metis conclusion\<^sub>G ground_superpositionI(12) premise\<^sub>1 premise\<^sub>1_\<gamma> premise\<^sub>2 premise\<^sub>2_\<gamma> special_case to_clause_inverse)
 
   obtain term\<^sub>2'_with_context where
     term\<^sub>2'_with_context: 
-    "term\<^sub>2'_with_context \<cdot>t \<theta> = (to_context context\<^sub>G)\<langle>to_term term\<^sub>G\<^sub>3\<rangle>"
+    "term\<^sub>2'_with_context \<cdot>t \<gamma> = (to_context context\<^sub>G)\<langle>to_term term\<^sub>G\<^sub>3\<rangle>"
     "term\<^sub>2'_with_context = (context\<^sub>1 \<cdot>t\<^sub>c \<rho>\<^sub>1)\<langle>term\<^sub>2' \<cdot>t \<rho>\<^sub>2\<rangle>" 
-    unfolding term\<^sub>2'_\<theta>[symmetric]  context\<^sub>1_\<theta>[symmetric]
+    unfolding term\<^sub>2'_\<gamma>[symmetric]  context\<^sub>1_\<gamma>[symmetric]
     by force
 
-  have term_term': "term\<^sub>1 \<cdot>t \<rho>\<^sub>1 \<cdot>t \<theta> = term\<^sub>2 \<cdot>t \<rho>\<^sub>2 \<cdot>t \<theta>"
-    unfolding term\<^sub>1_\<theta> term\<^sub>2_\<theta>
+  have term_term': "term\<^sub>1 \<cdot>t \<rho>\<^sub>1 \<cdot>t \<gamma> = term\<^sub>2 \<cdot>t \<rho>\<^sub>2 \<cdot>t \<gamma>"
+    unfolding term\<^sub>1_\<gamma> term\<^sub>2_\<gamma>
     by(rule refl)
 
-  then obtain \<sigma> \<tau> where \<sigma>: "term_subst.is_imgu \<sigma> {{term\<^sub>1 \<cdot>t \<rho>\<^sub>1, term\<^sub>2 \<cdot>t \<rho>\<^sub>2}}" "\<theta> = \<sigma> \<odot> \<tau>"
+  then obtain \<mu> \<sigma> where \<mu>: "term_subst.is_imgu \<mu> {{term\<^sub>1 \<cdot>t \<rho>\<^sub>1, term\<^sub>2 \<cdot>t \<rho>\<^sub>2}}" "\<gamma> = \<mu> \<odot> \<sigma>"
     using imgu_exists
     by blast
 
   let ?conclusion' = "add_mset (?\<P> (Upair (term\<^sub>2'_with_context) (term\<^sub>1' \<cdot>t \<rho>\<^sub>1))) 
-        (premise\<^sub>1' \<cdot> \<rho>\<^sub>1 + premise\<^sub>2' \<cdot> \<rho>\<^sub>2) \<cdot> \<sigma>"
+        (premise\<^sub>1' \<cdot> \<rho>\<^sub>1 + premise\<^sub>2' \<cdot> \<rho>\<^sub>2) \<cdot> \<mu>"
 
-  have "term_subst.is_idem \<sigma>"
-    using \<sigma>(1)
+  have "term_subst.is_idem \<mu>"
+    using \<mu>(1)
     by (simp add: term_subst.is_imgu_iff_is_idem_and_is_mgu)  
 
-  then have \<sigma>_\<theta>: "\<sigma> \<odot> \<theta> = \<theta>"
-    unfolding \<sigma>(2) term_subst.is_idem_def
+  then have \<mu>_\<gamma>: "\<mu> \<odot> \<gamma> = \<gamma>"
+    unfolding \<mu>(2) term_subst.is_idem_def
     by (metis subst_compose_assoc)
 
-  from conclusion_\<theta>\<^sub>G have conclusion_\<theta>: "conclusion \<cdot> \<theta> =  ?conclusion' \<cdot> \<theta>"
+  from conclusion_\<gamma>\<^sub>G have conclusion_\<gamma>: "conclusion \<cdot> \<gamma> =  ?conclusion' \<cdot> \<gamma>"
     unfolding 
       term\<^sub>2'_with_context[symmetric]
-      premise\<^sub>1'_\<theta>[symmetric] 
-      premise\<^sub>2'_\<theta>[symmetric] 
-      term\<^sub>1'_\<theta>[symmetric]
+      premise\<^sub>1'_\<gamma>[symmetric] 
+      premise\<^sub>2'_\<gamma>[symmetric] 
+      term\<^sub>1'_\<gamma>[symmetric]
       subst_clause_plus[symmetric] 
       subst_apply_term_ctxt_apply_distrib[symmetric]
       subst_atom[symmetric]
     apply(cases "\<P>\<^sub>G = Pos")
-    using subst_clause_add_mset subst_literal \<sigma>_\<theta> clause_subst_compose
+    using subst_clause_add_mset subst_literal \<mu>_\<gamma> clause_subst_compose
     by (smt (verit, del_insts))+
 
   have superposition: "superposition premise\<^sub>2 premise\<^sub>1 ?conclusion'"
@@ -1026,27 +1029,27 @@ proof(cases premise\<^sub>G\<^sub>2 premise\<^sub>G\<^sub>1 conclusion\<^sub>G r
     show "is_Fun term\<^sub>1"
       using term\<^sub>1_not_Var.
   next
-    show "term_subst.is_imgu \<sigma> {{term\<^sub>1 \<cdot>t \<rho>\<^sub>1, term\<^sub>2 \<cdot>t \<rho>\<^sub>2}}"
-      using \<sigma>(1).
+    show "term_subst.is_imgu \<mu> {{term\<^sub>1 \<cdot>t \<rho>\<^sub>1, term\<^sub>2 \<cdot>t \<rho>\<^sub>2}}"
+      using \<mu>(1).
   next
     note premises_to_ground_clause_inverse = assms(9, 10)[THEN to_ground_clause_inverse]  
-    note premise_groundings = assms(10, 9)[unfolded \<sigma>(2) clause_subst_compose]
+    note premise_groundings = assms(10, 9)[unfolded \<mu>(2) clause_subst_compose]
 
-    have "premise\<^sub>2 \<cdot> \<rho>\<^sub>2 \<cdot> \<sigma> \<cdot> \<tau> \<prec>\<^sub>c premise\<^sub>1 \<cdot> \<rho>\<^sub>1 \<cdot> \<sigma> \<cdot> \<tau>"
+    have "premise\<^sub>2 \<cdot> \<rho>\<^sub>2 \<cdot> \<mu> \<cdot> \<sigma> \<prec>\<^sub>c premise\<^sub>1 \<cdot> \<rho>\<^sub>1 \<cdot> \<mu> \<cdot> \<sigma>"
       using ground_superpositionI(3)[
           unfolded premise\<^sub>G\<^sub>1 premise\<^sub>G\<^sub>2 less\<^sub>c\<^sub>G_less\<^sub>c premises_to_ground_clause_inverse, 
-          unfolded \<sigma>(2) clause_subst_compose
+          unfolded \<mu>(2) clause_subst_compose
           ].
 
-    then show "\<not> premise\<^sub>1 \<cdot> \<rho>\<^sub>1 \<cdot> \<sigma> \<preceq>\<^sub>c premise\<^sub>2 \<cdot> \<rho>\<^sub>2 \<cdot> \<sigma>"
+    then show "\<not> premise\<^sub>1 \<cdot> \<rho>\<^sub>1 \<cdot> \<mu> \<preceq>\<^sub>c premise\<^sub>2 \<cdot> \<rho>\<^sub>2 \<cdot> \<mu>"
       using less\<^sub>c_less_eq\<^sub>c_ground_subst_stability[OF premise_groundings]
       by blast
   next
     show "?\<P> = Pos 
             \<and> select premise\<^sub>1 = {#} 
-            \<and> is_strictly_maximal\<^sub>l (literal\<^sub>1 \<cdot>l \<rho>\<^sub>1 \<cdot>l \<sigma>) (premise\<^sub>1 \<cdot> \<rho>\<^sub>1 \<cdot> \<sigma>) 
+            \<and> is_strictly_maximal\<^sub>l (literal\<^sub>1 \<cdot>l \<rho>\<^sub>1 \<cdot>l \<mu>) (premise\<^sub>1 \<cdot> \<rho>\<^sub>1 \<cdot> \<mu>) 
        \<or> ?\<P> = Neg 
-            \<and> (select premise\<^sub>1 = {#} \<and> is_maximal\<^sub>l (literal\<^sub>1 \<cdot>l \<rho>\<^sub>1 \<cdot>l \<sigma>) (premise\<^sub>1 \<cdot> \<rho>\<^sub>1 \<cdot> \<sigma>) 
+            \<and> (select premise\<^sub>1 = {#} \<and> is_maximal\<^sub>l (literal\<^sub>1 \<cdot>l \<rho>\<^sub>1 \<cdot>l \<mu>) (premise\<^sub>1 \<cdot> \<rho>\<^sub>1 \<cdot> \<mu>) 
                \<or> is_maximal\<^sub>l literal\<^sub>1 (select premise\<^sub>1))"
     proof(cases "?\<P> = Pos")
       case True
@@ -1054,16 +1057,16 @@ proof(cases premise\<^sub>G\<^sub>2 premise\<^sub>G\<^sub>1 conclusion\<^sub>G r
         using clause_subst_empty select(1) ground_superpositionI(9) 
         by(auto simp: subst_clause_def)
 
-      moreover have "is_strictly_maximal\<^sub>l (literal\<^sub>1 \<cdot>l \<rho>\<^sub>1 \<cdot>l \<sigma> \<cdot>l \<tau>) (premise\<^sub>1 \<cdot> \<rho>\<^sub>1 \<cdot> \<sigma> \<cdot> \<tau>)"
+      moreover have "is_strictly_maximal\<^sub>l (literal\<^sub>1 \<cdot>l \<rho>\<^sub>1 \<cdot>l \<mu> \<cdot>l \<sigma>) (premise\<^sub>1 \<cdot> \<rho>\<^sub>1 \<cdot> \<mu> \<cdot> \<sigma>)"
         using True pos_literal\<^sub>G\<^sub>1_is_strictly_maximal\<^sub>l
-        unfolding literal\<^sub>1_\<theta>[symmetric] \<sigma>(2)
+        unfolding literal\<^sub>1_\<gamma>[symmetric] \<mu>(2)
         by force
 
-      moreover then have "is_strictly_maximal\<^sub>l (literal\<^sub>1 \<cdot>l \<rho>\<^sub>1 \<cdot>l \<sigma>) (premise\<^sub>1 \<cdot> \<rho>\<^sub>1 \<cdot> \<sigma>)"
+      moreover then have "is_strictly_maximal\<^sub>l (literal\<^sub>1 \<cdot>l \<rho>\<^sub>1 \<cdot>l \<mu>) (premise\<^sub>1 \<cdot> \<rho>\<^sub>1 \<cdot> \<mu>)"
         using 
           is_strictly_maximal\<^sub>l_ground_subst_stability'[OF
             _
-            premise\<^sub>1_grounding[unfolded \<sigma>(2) clause_subst_compose]
+            premise\<^sub>1_grounding[unfolded \<mu>(2) clause_subst_compose]
             ]
           literal_in_clause_subst
           literal\<^sub>1_in_premise\<^sub>1
@@ -1085,16 +1088,16 @@ proof(cases premise\<^sub>G\<^sub>2 premise\<^sub>G\<^sub>1 conclusion\<^sub>G r
           using clause_subst_empty select(1) ground_superpositionI(9) \<P>\<^sub>G_Neg
           by auto
 
-        moreover have "is_maximal\<^sub>l (literal\<^sub>1 \<cdot>l \<rho>\<^sub>1 \<cdot>l \<sigma> \<cdot>l \<tau>) (premise\<^sub>1 \<cdot> \<rho>\<^sub>1 \<cdot> \<sigma> \<cdot> \<tau>)"
+        moreover have "is_maximal\<^sub>l (literal\<^sub>1 \<cdot>l \<rho>\<^sub>1 \<cdot>l \<mu> \<cdot>l \<sigma>) (premise\<^sub>1 \<cdot> \<rho>\<^sub>1 \<cdot> \<mu> \<cdot> \<sigma>)"
           using neg_literal\<^sub>G\<^sub>1_is_maximal\<^sub>l[OF \<P>\<^sub>G_Neg select\<^sub>G_empty]
-          unfolding literal\<^sub>1_\<theta>[symmetric] \<sigma>(2)
+          unfolding literal\<^sub>1_\<gamma>[symmetric] \<mu>(2)
           by simp
 
-        moreover then have "is_maximal\<^sub>l (literal\<^sub>1 \<cdot>l \<rho>\<^sub>1 \<cdot>l \<sigma>) (premise\<^sub>1 \<cdot> \<rho>\<^sub>1 \<cdot> \<sigma>)"
+        moreover then have "is_maximal\<^sub>l (literal\<^sub>1 \<cdot>l \<rho>\<^sub>1 \<cdot>l \<mu>) (premise\<^sub>1 \<cdot> \<rho>\<^sub>1 \<cdot> \<mu>)"
           using 
             is_maximal\<^sub>l_ground_subst_stability'[OF 
               _  
-              premise\<^sub>1_grounding[unfolded \<sigma>(2) clause_subst_compose]
+              premise\<^sub>1_grounding[unfolded \<mu>(2) clause_subst_compose]
               ]
             literal_in_clause_subst
             literal\<^sub>1_in_premise\<^sub>1
@@ -1117,107 +1120,107 @@ proof(cases premise\<^sub>G\<^sub>2 premise\<^sub>G\<^sub>1 conclusion\<^sub>G r
       using clause_subst_empty ground_superpositionI(10) select(2)
       by auto
   next 
-    have "is_strictly_maximal\<^sub>l (literal\<^sub>2 \<cdot>l \<rho>\<^sub>2 \<cdot>l \<sigma> \<cdot>l \<tau>) (premise\<^sub>2 \<cdot> \<rho>\<^sub>2 \<cdot> \<sigma> \<cdot> \<tau>)"
+    have "is_strictly_maximal\<^sub>l (literal\<^sub>2 \<cdot>l \<rho>\<^sub>2 \<cdot>l \<mu> \<cdot>l \<sigma>) (premise\<^sub>2 \<cdot> \<rho>\<^sub>2 \<cdot> \<mu> \<cdot> \<sigma>)"
       using literal\<^sub>G\<^sub>2_is_strictly_maximal\<^sub>l
-      unfolding literal\<^sub>2_\<theta>[symmetric]  \<sigma>(2)
+      unfolding literal\<^sub>2_\<gamma>[symmetric]  \<mu>(2)
       by simp
 
-    then show "is_strictly_maximal\<^sub>l (literal\<^sub>2 \<cdot>l \<rho>\<^sub>2 \<cdot>l \<sigma>) (premise\<^sub>2 \<cdot> \<rho>\<^sub>2 \<cdot> \<sigma>)"
+    then show "is_strictly_maximal\<^sub>l (literal\<^sub>2 \<cdot>l \<rho>\<^sub>2 \<cdot>l \<mu>) (premise\<^sub>2 \<cdot> \<rho>\<^sub>2 \<cdot> \<mu>)"
       using 
         is_strictly_maximal\<^sub>l_ground_subst_stability'[OF 
-          _  premise\<^sub>2_grounding[unfolded \<sigma>(2) clause_subst_compose]
+          _  premise\<^sub>2_grounding[unfolded \<mu>(2) clause_subst_compose]
           ]
         literal\<^sub>2_in_premise\<^sub>2 
         literal_in_clause_subst 
       by blast
   next
     have term_groundings: 
-      "is_ground_term (term\<^sub>1' \<cdot>t \<rho>\<^sub>1 \<cdot>t \<sigma> \<cdot>t \<tau>)" 
-      "is_ground_term (context\<^sub>1\<langle>term\<^sub>1\<rangle> \<cdot>t \<rho>\<^sub>1 \<cdot>t \<sigma> \<cdot>t \<tau>)" 
+      "is_ground_term (term\<^sub>1' \<cdot>t \<rho>\<^sub>1 \<cdot>t \<mu> \<cdot>t \<sigma>)" 
+      "is_ground_term (context\<^sub>1\<langle>term\<^sub>1\<rangle> \<cdot>t \<rho>\<^sub>1 \<cdot>t \<mu> \<cdot>t \<sigma>)" 
       unfolding 
         term\<^sub>1_with_context[symmetric]  
-        term\<^sub>1_with_context_\<theta>[unfolded \<sigma>(2) term_subst_compose]
-        term\<^sub>1'_\<theta>[unfolded \<sigma>(2) term_subst_compose]
+        term\<^sub>1_with_context_\<gamma>[unfolded \<mu>(2) term_subst_compose]
+        term\<^sub>1'_\<gamma>[unfolded \<mu>(2) term_subst_compose]
       using ground_term_with_context_is_ground(1)
       by simp_all
 
-    have "term\<^sub>1' \<cdot>t \<rho>\<^sub>1 \<cdot>t \<sigma> \<cdot>t \<tau> \<prec>\<^sub>t context\<^sub>1\<langle>term\<^sub>1\<rangle> \<cdot>t \<rho>\<^sub>1 \<cdot>t \<sigma> \<cdot>t \<tau>"
+    have "term\<^sub>1' \<cdot>t \<rho>\<^sub>1 \<cdot>t \<mu> \<cdot>t \<sigma> \<prec>\<^sub>t context\<^sub>1\<langle>term\<^sub>1\<rangle> \<cdot>t \<rho>\<^sub>1 \<cdot>t \<mu> \<cdot>t \<sigma>"
       using ground_superpositionI(7) 
       unfolding 
-        term\<^sub>1'_\<theta>[unfolded \<sigma>(2) term_subst_compose]
+        term\<^sub>1'_\<gamma>[unfolded \<mu>(2) term_subst_compose]
         term\<^sub>1_with_context[symmetric]
-        term\<^sub>1_with_context_\<theta>[unfolded \<sigma>(2) term_subst_compose]
+        term\<^sub>1_with_context_\<gamma>[unfolded \<mu>(2) term_subst_compose]
         less\<^sub>t\<^sub>G_def
         ground_term_with_context(3).
 
-    then show "\<not> context\<^sub>1\<langle>term\<^sub>1\<rangle> \<cdot>t \<rho>\<^sub>1 \<cdot>t \<sigma> \<preceq>\<^sub>t term\<^sub>1' \<cdot>t \<rho>\<^sub>1 \<cdot>t \<sigma>"
+    then show "\<not> context\<^sub>1\<langle>term\<^sub>1\<rangle> \<cdot>t \<rho>\<^sub>1 \<cdot>t \<mu> \<preceq>\<^sub>t term\<^sub>1' \<cdot>t \<rho>\<^sub>1 \<cdot>t \<mu>"
       using less\<^sub>t_less_eq\<^sub>t_ground_subst_stability[OF term_groundings]
       by blast
   next
     have term_groundings: 
-      "is_ground_term (term\<^sub>2' \<cdot>t \<rho>\<^sub>2 \<cdot>t \<sigma> \<cdot>t \<tau>)" 
-      "is_ground_term (term\<^sub>2 \<cdot>t \<rho>\<^sub>2 \<cdot>t \<sigma> \<cdot>t \<tau>)" 
+      "is_ground_term (term\<^sub>2' \<cdot>t \<rho>\<^sub>2 \<cdot>t \<mu> \<cdot>t \<sigma>)" 
+      "is_ground_term (term\<^sub>2 \<cdot>t \<rho>\<^sub>2 \<cdot>t \<mu> \<cdot>t \<sigma>)" 
       unfolding 
-        term\<^sub>2_\<theta>[unfolded \<sigma>(2) term_subst_compose]
-        term\<^sub>2'_\<theta>[unfolded \<sigma>(2) term_subst_compose]
+        term\<^sub>2_\<gamma>[unfolded \<mu>(2) term_subst_compose]
+        term\<^sub>2'_\<gamma>[unfolded \<mu>(2) term_subst_compose]
       by simp_all
 
-    have "term\<^sub>2' \<cdot>t \<rho>\<^sub>2 \<cdot>t \<sigma> \<cdot>t \<tau> \<prec>\<^sub>t term\<^sub>2 \<cdot>t \<rho>\<^sub>2 \<cdot>t \<sigma> \<cdot>t \<tau>"
+    have "term\<^sub>2' \<cdot>t \<rho>\<^sub>2 \<cdot>t \<mu> \<cdot>t \<sigma> \<prec>\<^sub>t term\<^sub>2 \<cdot>t \<rho>\<^sub>2 \<cdot>t \<mu> \<cdot>t \<sigma>"
       using ground_superpositionI(8) 
       unfolding 
-        term\<^sub>2_\<theta>[unfolded \<sigma>(2) term_subst_compose]             
-        term\<^sub>2'_\<theta>[unfolded \<sigma>(2) term_subst_compose]
+        term\<^sub>2_\<gamma>[unfolded \<mu>(2) term_subst_compose]             
+        term\<^sub>2'_\<gamma>[unfolded \<mu>(2) term_subst_compose]
         less\<^sub>t\<^sub>G_def.
 
-    then show "\<not> term\<^sub>2 \<cdot>t \<rho>\<^sub>2 \<cdot>t \<sigma> \<preceq>\<^sub>t term\<^sub>2' \<cdot>t \<rho>\<^sub>2 \<cdot>t \<sigma>"
+    then show "\<not> term\<^sub>2 \<cdot>t \<rho>\<^sub>2 \<cdot>t \<mu> \<preceq>\<^sub>t term\<^sub>2' \<cdot>t \<rho>\<^sub>2 \<cdot>t \<mu>"
       using less\<^sub>t_less_eq\<^sub>t_ground_subst_stability[OF term_groundings]
       by blast
   next
     show "?conclusion' =  add_mset
      ((if \<P>\<^sub>G = Pos then Pos else Neg) (Upair (context\<^sub>1 \<cdot>t\<^sub>c \<rho>\<^sub>1)\<langle>term\<^sub>2' \<cdot>t \<rho>\<^sub>2\<rangle> (term\<^sub>1' \<cdot>t \<rho>\<^sub>1)))
-     (premise\<^sub>1' \<cdot> \<rho>\<^sub>1 + premise\<^sub>2' \<cdot> \<rho>\<^sub>2) \<cdot> \<sigma>"
+     (premise\<^sub>1' \<cdot> \<rho>\<^sub>1 + premise\<^sub>2' \<cdot> \<rho>\<^sub>2) \<cdot> \<mu>"
       using term\<^sub>2'_with_context(2) by blast
   qed
 
-  have "term_subst.is_idem \<sigma>"
-    using \<sigma>(1)
+  have "term_subst.is_idem \<mu>"
+    using \<mu>(1)
     by (simp add: term_subst.is_imgu_iff_is_idem_and_is_mgu)  
 
-  then have \<sigma>_\<theta>: "\<sigma> \<odot> \<theta> = \<theta>"
-    unfolding \<sigma>(2) term_subst.is_idem_def
+  then have \<mu>_\<gamma>: "\<mu> \<odot> \<gamma> = \<gamma>"
+    unfolding \<mu>(2) term_subst.is_idem_def
     by (metis subst_compose_assoc)
 
-  have "to_ground_clause (premise\<^sub>1 \<cdot> \<rho>\<^sub>1 \<cdot> \<theta>) \<in> clause_groundings premise\<^sub>1"
+  have "to_ground_clause (premise\<^sub>1 \<cdot> \<rho>\<^sub>1 \<cdot> \<gamma>) \<in> clause_groundings premise\<^sub>1"
     unfolding clause_groundings_def
     by (smt (verit, del_insts) clause_subst_compose mem_Collect_eq premise\<^sub>1_grounding)
 
-  moreover have "to_ground_clause (premise\<^sub>2 \<cdot> \<rho>\<^sub>2 \<cdot> \<theta>) \<in> clause_groundings premise\<^sub>2"
+  moreover have "to_ground_clause (premise\<^sub>2 \<cdot> \<rho>\<^sub>2 \<cdot> \<gamma>) \<in> clause_groundings premise\<^sub>2"
     unfolding clause_groundings_def
     by (smt (verit, del_insts) clause_subst_compose mem_Collect_eq premise\<^sub>2_grounding)
 
-  moreover have "conclusion \<cdot> \<theta> = 
+  moreover have "conclusion \<cdot> \<gamma> = 
     add_mset (?\<P> (Upair (to_context context\<^sub>G)\<langle>to_term term\<^sub>G\<^sub>3\<rangle> (to_term term\<^sub>G\<^sub>2))) 
       (to_clause premise\<^sub>G\<^sub>1' + to_clause premise\<^sub>G\<^sub>2')"
     using ground_superpositionI(4, 12) to_ground_clause_inverse[OF conclusion_grounding] 
     unfolding ground_term_with_context(3) to_term_to_atom
     by(cases "\<P>\<^sub>G = Pos")(simp_all add: to_atom_to_literal to_clause_add_mset)
 
-  then have conclusion_\<theta>: "conclusion \<cdot> \<theta> =  ?conclusion' \<cdot> \<theta>"
+  then have conclusion_\<gamma>: "conclusion \<cdot> \<gamma> =  ?conclusion' \<cdot> \<gamma>"
     unfolding 
       term\<^sub>2'_with_context[symmetric]
-      premise\<^sub>1'_\<theta>[symmetric] 
-      premise\<^sub>2'_\<theta>[symmetric] 
-      term\<^sub>1'_\<theta>[symmetric]
+      premise\<^sub>1'_\<gamma>[symmetric] 
+      premise\<^sub>2'_\<gamma>[symmetric] 
+      term\<^sub>1'_\<gamma>[symmetric]
       subst_clause_plus[symmetric] 
       subst_apply_term_ctxt_apply_distrib[symmetric]
       subst_atom[symmetric]
     apply(cases "\<P>\<^sub>G = Pos")
-    using subst_clause_add_mset subst_literal \<sigma>_\<theta> clause_subst_compose
+    using subst_clause_add_mset subst_literal \<mu>_\<gamma> clause_subst_compose
     by (smt (verit))+
 
-  have "to_ground_clause (conclusion \<cdot> \<theta>) \<in> clause_groundings ?conclusion'"
+  have "to_ground_clause (conclusion \<cdot> \<gamma>) \<in> clause_groundings ?conclusion'"
     unfolding clause_groundings_def
-    by (smt (verit, best) conclusion_\<theta> conclusion_grounding mem_Collect_eq)
+    by (smt (verit, best) conclusion_\<gamma> conclusion_grounding mem_Collect_eq)
 
 (* TODO: *)
   ultimately show ?thesis
@@ -1225,14 +1228,14 @@ proof(cases premise\<^sub>G\<^sub>2 premise\<^sub>G\<^sub>1 conclusion\<^sub>G r
     unfolding clause_groundings_def inference_groundings_def ground.G_Inf_def inferences_def
     using superposition
     apply simp
-    by (metis conclusion\<^sub>G conclusion_\<theta> conclusion_grounding ground_superposition premise\<^sub>1_grounding premise\<^sub>2_grounding premise\<^sub>G\<^sub>1 premise\<^sub>G\<^sub>2 renaming(1) renaming(2) renaming(3))
+    by (metis conclusion\<^sub>G conclusion_\<gamma> conclusion_grounding ground_superposition premise\<^sub>1_grounding premise\<^sub>2_grounding premise\<^sub>G\<^sub>1 premise\<^sub>G\<^sub>2 renaming(1) renaming(2) renaming(3))
 qed
 
 abbreviation subst_stability_on where
   "subst_stability_on premises \<equiv>
-    \<forall>premise\<^sub>G \<in> \<Union> (clause_groundings ` premises). \<exists>premise \<in> premises. \<exists>\<theta>. 
-          premise \<cdot> \<theta> = to_clause premise\<^sub>G 
-        \<and> to_clause (select\<^sub>G (to_ground_clause (premise \<cdot> \<theta>))) = (select premise) \<cdot> \<theta>"
+    \<forall>premise\<^sub>G \<in> \<Union> (clause_groundings ` premises). \<exists>premise \<in> premises. \<exists>\<gamma>. 
+          premise \<cdot> \<gamma> = to_clause premise\<^sub>G 
+        \<and> to_clause (select\<^sub>G (to_ground_clause (premise \<cdot> \<gamma>))) = (select premise) \<cdot> \<gamma>"
 
 lemma eq_resolution_ground_instance': 
   assumes 
@@ -1252,28 +1255,28 @@ proof-
     unfolding \<iota>\<^sub>G ground.Inf_from_q_def ground.Inf_from_def
     by simp
 
-  obtain premise conclusion \<theta> where
-    "to_clause premise\<^sub>G = premise \<cdot> \<theta>" and
-    "to_clause conclusion\<^sub>G = conclusion \<cdot> \<theta>" and
-    select: "to_clause (select\<^sub>G premise\<^sub>G) = select premise \<cdot> \<theta>" and
+  obtain premise conclusion \<gamma> where
+    "to_clause premise\<^sub>G = premise \<cdot> \<gamma>" and
+    "to_clause conclusion\<^sub>G = conclusion \<cdot> \<gamma>" and
+    select: "to_clause (select\<^sub>G premise\<^sub>G) = select premise \<cdot> \<gamma>" and
     premise_in_premises: "premise \<in> premises"
     using assms(2, 3) premise\<^sub>G_in_groundings
     unfolding \<iota>\<^sub>G ground.Inf_from_q_def ground.Inf_from_def 
     by (metis (no_types, opaque_lifting) ground_clause_is_ground subst_ground_clause to_clause_inverse)
 
   then have 
-    premise_grounding: "is_ground_clause (premise \<cdot> \<theta>)" and 
-    premise\<^sub>G: "premise\<^sub>G = to_ground_clause (premise \<cdot> \<theta>)" and 
-    conclusion_grounding: "is_ground_clause (conclusion \<cdot> \<theta>)" and
-    conclusion\<^sub>G: "conclusion\<^sub>G = to_ground_clause (conclusion \<cdot> \<theta>)"
+    premise_grounding: "is_ground_clause (premise \<cdot> \<gamma>)" and 
+    premise\<^sub>G: "premise\<^sub>G = to_ground_clause (premise \<cdot> \<gamma>)" and 
+    conclusion_grounding: "is_ground_clause (conclusion \<cdot> \<gamma>)" and
+    conclusion\<^sub>G: "conclusion\<^sub>G = to_ground_clause (conclusion \<cdot> \<gamma>)"
     by (smt ground_clause_is_ground to_clause_inverse)+
 
   obtain conclusion' where 
     eq_resolution: "eq_resolution premise conclusion'" and
     inference_groundings: 
-    "Infer [to_ground_clause (premise \<cdot> \<theta>)] (to_ground_clause (conclusion' \<cdot> \<theta>)) \<in> 
+    "Infer [to_ground_clause (premise \<cdot> \<gamma>)] (to_ground_clause (conclusion' \<cdot> \<gamma>)) \<in> 
         inference_groundings (Infer [premise] conclusion')" and  
-    conclusion'_conclusion: "conclusion' \<cdot> \<theta> = conclusion \<cdot> \<theta>"
+    conclusion'_conclusion: "conclusion' \<cdot> \<gamma> = conclusion \<cdot> \<gamma>"
     using 
       premise_grounding 
       conclusion_grounding 
@@ -1318,28 +1321,28 @@ proof-
     unfolding \<iota>\<^sub>G ground.Inf_from_q_def ground.Inf_from_def
     by simp
 
-  obtain premise conclusion \<theta> where
-    "to_clause premise\<^sub>G = premise \<cdot> \<theta>" and
-    "to_clause conclusion\<^sub>G = conclusion \<cdot> \<theta>" and
-    select: "to_clause (select\<^sub>G (to_ground_clause (premise \<cdot> \<theta>))) = select premise \<cdot> \<theta>" and
+  obtain premise conclusion \<gamma> where
+    "to_clause premise\<^sub>G = premise \<cdot> \<gamma>" and
+    "to_clause conclusion\<^sub>G = conclusion \<cdot> \<gamma>" and
+    select: "to_clause (select\<^sub>G (to_ground_clause (premise \<cdot> \<gamma>))) = select premise \<cdot> \<gamma>" and
     premise_in_premises: "premise \<in> premises"
     using assms(2, 3) premise\<^sub>G_in_groundings
     unfolding \<iota>\<^sub>G ground.Inf_from_q_def ground.Inf_from_def
     by (metis (no_types, opaque_lifting) ground_clause_is_ground subst_ground_clause)
 
   then have 
-    premise_grounding: "is_ground_clause (premise \<cdot> \<theta>)" and 
-    premise\<^sub>G: "premise\<^sub>G = to_ground_clause (premise \<cdot> \<theta>)" and 
-    conclusion_grounding: "is_ground_clause (conclusion \<cdot> \<theta>)" and
-    conclusion\<^sub>G: "conclusion\<^sub>G = to_ground_clause (conclusion \<cdot> \<theta>)"
+    premise_grounding: "is_ground_clause (premise \<cdot> \<gamma>)" and 
+    premise\<^sub>G: "premise\<^sub>G = to_ground_clause (premise \<cdot> \<gamma>)" and 
+    conclusion_grounding: "is_ground_clause (conclusion \<cdot> \<gamma>)" and
+    conclusion\<^sub>G: "conclusion\<^sub>G = to_ground_clause (conclusion \<cdot> \<gamma>)"
     by (smt ground_clause_is_ground to_clause_inverse)+
 
   obtain conclusion' where 
     eq_factoring: "eq_factoring premise conclusion'" and
     inference_groundings: 
-    "Infer [to_ground_clause (premise \<cdot> \<theta>)] (to_ground_clause (conclusion' \<cdot> \<theta>)) \<in> 
+    "Infer [to_ground_clause (premise \<cdot> \<gamma>)] (to_ground_clause (conclusion' \<cdot> \<gamma>)) \<in> 
         inference_groundings (Infer [premise] conclusion')" and  
-    conclusion'_conclusion: "conclusion' \<cdot> \<theta> = conclusion \<cdot> \<theta>"
+    conclusion'_conclusion: "conclusion' \<cdot> \<gamma> = conclusion \<cdot> \<gamma>"
     using 
       eq_factoring_lifting[OF 
         premise_grounding 
@@ -1385,12 +1388,12 @@ proof-
     unfolding \<iota>\<^sub>G ground.Inf_from_q_def ground.Inf_from_def
     by simp_all
 
-  obtain premise\<^sub>1 premise\<^sub>2 \<theta>\<^sub>1 \<theta>\<^sub>2 where
-    premise\<^sub>1_\<theta>\<^sub>1: "premise\<^sub>1 \<cdot> \<theta>\<^sub>1 = to_clause premise\<^sub>G\<^sub>1" and
-    premise\<^sub>2_\<theta>\<^sub>2: "premise\<^sub>2 \<cdot> \<theta>\<^sub>2 = to_clause premise\<^sub>G\<^sub>2" and
+  obtain premise\<^sub>1 premise\<^sub>2 \<gamma>\<^sub>1 \<gamma>\<^sub>2 where
+    premise\<^sub>1_\<gamma>\<^sub>1: "premise\<^sub>1 \<cdot> \<gamma>\<^sub>1 = to_clause premise\<^sub>G\<^sub>1" and
+    premise\<^sub>2_\<gamma>\<^sub>2: "premise\<^sub>2 \<cdot> \<gamma>\<^sub>2 = to_clause premise\<^sub>G\<^sub>2" and
     select': 
-    "to_clause (select\<^sub>G (to_ground_clause (premise\<^sub>1 \<cdot> \<theta>\<^sub>1))) = select premise\<^sub>1 \<cdot> \<theta>\<^sub>1"
-    "to_clause (select\<^sub>G (to_ground_clause (premise\<^sub>2 \<cdot> \<theta>\<^sub>2))) = select premise\<^sub>2 \<cdot> \<theta>\<^sub>2" and
+    "to_clause (select\<^sub>G (to_ground_clause (premise\<^sub>1 \<cdot> \<gamma>\<^sub>1))) = select premise\<^sub>1 \<cdot> \<gamma>\<^sub>1"
+    "to_clause (select\<^sub>G (to_ground_clause (premise\<^sub>2 \<cdot> \<gamma>\<^sub>2))) = select premise\<^sub>2 \<cdot> \<gamma>\<^sub>2" and
     premise\<^sub>1_in_premises: "premise\<^sub>1 \<in> premises" and
     premise\<^sub>2_in_premises: "premise\<^sub>2 \<in> premises"
     using assms(2, 4) premise\<^sub>G\<^sub>1_in_groundings premise\<^sub>G\<^sub>2_in_groundings
@@ -1428,56 +1431,56 @@ proof-
     using vars_distinct
     by blast
 
-  obtain \<theta> where "\<theta> = (\<lambda>var. 
+  obtain \<gamma> where "\<gamma> = (\<lambda>var. 
       if var \<in> vars_clause (premise\<^sub>1 \<cdot> \<rho>\<^sub>1) 
-      then (\<rho>\<^sub>1_inv \<odot> \<theta>\<^sub>1) var 
-      else (\<rho>\<^sub>2_inv \<odot> \<theta>\<^sub>2) var
+      then (\<rho>\<^sub>1_inv \<odot> \<gamma>\<^sub>1) var 
+      else (\<rho>\<^sub>2_inv \<odot> \<gamma>\<^sub>2) var
     )"
     by simp
 
   then have 
-    premise\<^sub>1_\<theta>: "premise\<^sub>1 \<cdot> \<rho>\<^sub>1 \<cdot> \<theta> = to_clause premise\<^sub>G\<^sub>1" and
-    premise\<^sub>2_\<theta>: "premise\<^sub>2 \<cdot> \<rho>\<^sub>2 \<cdot> \<theta> = to_clause premise\<^sub>G\<^sub>2" and
+    premise\<^sub>1_\<gamma>: "premise\<^sub>1 \<cdot> \<rho>\<^sub>1 \<cdot> \<gamma> = to_clause premise\<^sub>G\<^sub>1" and
+    premise\<^sub>2_\<gamma>: "premise\<^sub>2 \<cdot> \<rho>\<^sub>2 \<cdot> \<gamma> = to_clause premise\<^sub>G\<^sub>2" and
     select: 
-    "to_clause (select\<^sub>G (to_ground_clause (premise\<^sub>1 \<cdot> \<rho>\<^sub>1 \<cdot> \<theta>))) = select premise\<^sub>1 \<cdot> \<rho>\<^sub>1 \<cdot> \<theta>"
-    "to_clause (select\<^sub>G (to_ground_clause (premise\<^sub>2 \<cdot> \<rho>\<^sub>2 \<cdot> \<theta>))) = select premise\<^sub>2 \<cdot> \<rho>\<^sub>2 \<cdot> \<theta>"
-    using premise\<^sub>1_\<theta>\<^sub>1 premise\<^sub>2_\<theta>\<^sub>2 select' 
-       apply auto
+    "to_clause (select\<^sub>G (to_ground_clause (premise\<^sub>1 \<cdot> \<rho>\<^sub>1 \<cdot> \<gamma>))) = select premise\<^sub>1 \<cdot> \<rho>\<^sub>1 \<cdot> \<gamma>"
+    "to_clause (select\<^sub>G (to_ground_clause (premise\<^sub>2 \<cdot> \<rho>\<^sub>2 \<cdot> \<gamma>))) = select premise\<^sub>2 \<cdot> \<rho>\<^sub>2 \<cdot> \<gamma>"
+    using premise\<^sub>1_\<gamma>\<^sub>1 premise\<^sub>2_\<gamma>\<^sub>2 select' 
+    apply auto
 
     using \<rho>\<^sub>1_inv \<rho>\<^sub>2_inv 
-       apply (metis (mono_tags, lifting) clause_subst_compose subst_clause_Var_ident)
-      apply (metis \<rho>\<^sub>2_inv clause_subst_compose clause_subst_reduntant_if' inf_commute subst_clause_Var_ident vars_distinct)
+    apply (metis (mono_tags, lifting) clause_subst_compose subst_clause_Var_ident)
+    apply (metis \<rho>\<^sub>2_inv clause_subst_compose clause_subst_reduntant_if' inf_commute subst_clause_Var_ident vars_distinct)
     apply (metis (no_types, lifting) \<rho>\<^sub>1_inv a(1) clause_submset_vars_clause_subset clause_subst_compose clause_subst_eq select'(1) subset_eq subst_clause_Var_ident)
     by (metis Int_iff \<rho>\<^sub>2_inv all_not_in_conv b clause_subst_compose clause_subst_reduntant_if' subst_clause_Var_ident to_clause_inverse vars_distinct)
 
-  obtain conclusion where conclusion_\<theta>: "to_clause conclusion\<^sub>G = conclusion \<cdot> \<theta>"
+  obtain conclusion where conclusion_\<gamma>: "to_clause conclusion\<^sub>G = conclusion \<cdot> \<gamma>"
     by (metis ground_clause_is_ground subst_ground_clause)
 
   then have 
-    premise\<^sub>1_grounding: "is_ground_clause (premise\<^sub>1 \<cdot> \<rho>\<^sub>1 \<cdot> \<theta>)" and 
-    premise\<^sub>2_grounding: "is_ground_clause (premise\<^sub>2 \<cdot> \<rho>\<^sub>2 \<cdot> \<theta>)" and 
-    premise\<^sub>G\<^sub>1: "premise\<^sub>G\<^sub>1 = to_ground_clause (premise\<^sub>1 \<cdot> \<rho>\<^sub>1 \<cdot> \<theta>)" and 
-    premise\<^sub>G\<^sub>2: "premise\<^sub>G\<^sub>2 = to_ground_clause (premise\<^sub>2 \<cdot> \<rho>\<^sub>2 \<cdot> \<theta>)" and 
-    conclusion_grounding: "is_ground_clause (conclusion \<cdot> \<theta>)" and
-    conclusion\<^sub>G: "conclusion\<^sub>G = to_ground_clause (conclusion \<cdot> \<theta>)"
-    apply (simp_all add: premise\<^sub>1_\<theta> premise\<^sub>2_\<theta>)
+    premise\<^sub>1_grounding: "is_ground_clause (premise\<^sub>1 \<cdot> \<rho>\<^sub>1 \<cdot> \<gamma>)" and 
+    premise\<^sub>2_grounding: "is_ground_clause (premise\<^sub>2 \<cdot> \<rho>\<^sub>2 \<cdot> \<gamma>)" and 
+    premise\<^sub>G\<^sub>1: "premise\<^sub>G\<^sub>1 = to_ground_clause (premise\<^sub>1 \<cdot> \<rho>\<^sub>1 \<cdot> \<gamma>)" and 
+    premise\<^sub>G\<^sub>2: "premise\<^sub>G\<^sub>2 = to_ground_clause (premise\<^sub>2 \<cdot> \<rho>\<^sub>2 \<cdot> \<gamma>)" and 
+    conclusion_grounding: "is_ground_clause (conclusion \<cdot> \<gamma>)" and
+    conclusion\<^sub>G: "conclusion\<^sub>G = to_ground_clause (conclusion \<cdot> \<gamma>)"
+    apply (simp_all add: premise\<^sub>1_\<gamma> premise\<^sub>2_\<gamma>)
     by (smt ground_clause_is_ground to_clause_inverse)+
 
   have "clause_groundings premise\<^sub>1 \<union> clause_groundings premise\<^sub>2 \<subseteq> \<Union> (clause_groundings ` premises)"
     using premise\<^sub>1_in_premises premise\<^sub>2_in_premises by blast
 
   then have Infer_not_GRed_I:
-    "Infer [to_ground_clause (premise\<^sub>2 \<cdot> \<rho>\<^sub>2 \<cdot> \<theta>), to_ground_clause (premise\<^sub>1 \<cdot> \<rho>\<^sub>1 \<cdot> \<theta>)]
-      (to_ground_clause (conclusion \<cdot> \<theta>)) \<notin>
+    "Infer [to_ground_clause (premise\<^sub>2 \<cdot> \<rho>\<^sub>2 \<cdot> \<gamma>), to_ground_clause (premise\<^sub>1 \<cdot> \<rho>\<^sub>1 \<cdot> \<gamma>)]
+      (to_ground_clause (conclusion \<cdot> \<gamma>)) \<notin>
       ground.GRed_I (clause_groundings premise\<^sub>1 \<union> clause_groundings premise\<^sub>2)"
     using assms(3) ground.Red_I_of_subset
     unfolding \<iota>\<^sub>G  premise\<^sub>G\<^sub>1[symmetric] premise\<^sub>G\<^sub>2[symmetric] conclusion\<^sub>G[symmetric]
     by blast
 
   have "\<exists>conclusion'. superposition premise\<^sub>2 premise\<^sub>1 conclusion' \<and>
-    Infer [to_ground_clause (premise\<^sub>2 \<cdot> \<rho>\<^sub>2 \<cdot> \<theta>), to_ground_clause (premise\<^sub>1 \<cdot> \<rho>\<^sub>1 \<cdot> \<theta>)]
-      (to_ground_clause (conclusion' \<cdot> \<theta>)) \<in> inference_groundings (Infer [premise\<^sub>2, premise\<^sub>1] conclusion') \<and>
-    conclusion' \<cdot> \<theta> = conclusion \<cdot> \<theta>"
+    Infer [to_ground_clause (premise\<^sub>2 \<cdot> \<rho>\<^sub>2 \<cdot> \<gamma>), to_ground_clause (premise\<^sub>1 \<cdot> \<rho>\<^sub>1 \<cdot> \<gamma>)]
+      (to_ground_clause (conclusion' \<cdot> \<gamma>)) \<in> inference_groundings (Infer [premise\<^sub>2, premise\<^sub>1] conclusion') \<and>
+    conclusion' \<cdot> \<gamma> = conclusion \<cdot> \<gamma>"
   proof (rule superposition_lifting)
     show "term_subst.is_renaming \<rho>\<^sub>1"
       using renaming by argo
@@ -1488,29 +1491,29 @@ proof-
     show "vars_clause (premise\<^sub>1 \<cdot> \<rho>\<^sub>1) \<inter> vars_clause (premise\<^sub>2 \<cdot> \<rho>\<^sub>2) = {}"
       using vars_distinct .
   next
-    show "is_ground_clause (premise\<^sub>1 \<cdot> \<rho>\<^sub>1 \<cdot> \<theta>)"
+    show "is_ground_clause (premise\<^sub>1 \<cdot> \<rho>\<^sub>1 \<cdot> \<gamma>)"
       using premise\<^sub>1_grounding .
   next
-    show "is_ground_clause (premise\<^sub>2 \<cdot> \<rho>\<^sub>2 \<cdot> \<theta>)"
+    show "is_ground_clause (premise\<^sub>2 \<cdot> \<rho>\<^sub>2 \<cdot> \<gamma>)"
       using premise\<^sub>2_grounding .
   next
-    show "is_ground_clause (conclusion \<cdot> \<theta>)"
+    show "is_ground_clause (conclusion \<cdot> \<gamma>)"
       using conclusion_grounding .
   next
-    show "to_clause (select\<^sub>G (to_ground_clause (premise\<^sub>1 \<cdot> \<rho>\<^sub>1 \<cdot> \<theta>))) = select premise\<^sub>1 \<cdot> \<rho>\<^sub>1 \<cdot> \<theta>"
+    show "to_clause (select\<^sub>G (to_ground_clause (premise\<^sub>1 \<cdot> \<rho>\<^sub>1 \<cdot> \<gamma>))) = select premise\<^sub>1 \<cdot> \<rho>\<^sub>1 \<cdot> \<gamma>"
       using select by argo
   next
-    show "to_clause (select\<^sub>G (to_ground_clause (premise\<^sub>2 \<cdot> \<rho>\<^sub>2 \<cdot> \<theta>))) = select premise\<^sub>2 \<cdot> \<rho>\<^sub>2 \<cdot> \<theta>"
+    show "to_clause (select\<^sub>G (to_ground_clause (premise\<^sub>2 \<cdot> \<rho>\<^sub>2 \<cdot> \<gamma>))) = select premise\<^sub>2 \<cdot> \<rho>\<^sub>2 \<cdot> \<gamma>"
       using select by argo
   next
     show "ground.ground_superposition
-      (to_ground_clause (premise\<^sub>2 \<cdot> \<rho>\<^sub>2 \<cdot> \<theta>))
-      (to_ground_clause (premise\<^sub>1 \<cdot> \<rho>\<^sub>1 \<cdot> \<theta>))
-      (to_ground_clause (conclusion \<cdot> \<theta>))"
+      (to_ground_clause (premise\<^sub>2 \<cdot> \<rho>\<^sub>2 \<cdot> \<gamma>))
+      (to_ground_clause (premise\<^sub>1 \<cdot> \<rho>\<^sub>1 \<cdot> \<gamma>))
+      (to_ground_clause (conclusion \<cdot> \<gamma>))"
       using ground_superposition unfolding premise\<^sub>G\<^sub>2 premise\<^sub>G\<^sub>1 conclusion\<^sub>G .
   next
-    show "Infer [to_ground_clause (premise\<^sub>2 \<cdot> \<rho>\<^sub>2 \<cdot> \<theta>), to_ground_clause (premise\<^sub>1 \<cdot> \<rho>\<^sub>1 \<cdot> \<theta>)]
-     (to_ground_clause (conclusion \<cdot> \<theta>))
+    show "Infer [to_ground_clause (premise\<^sub>2 \<cdot> \<rho>\<^sub>2 \<cdot> \<gamma>), to_ground_clause (premise\<^sub>1 \<cdot> \<rho>\<^sub>1 \<cdot> \<gamma>)]
+     (to_ground_clause (conclusion \<cdot> \<gamma>))
     \<notin> ground.GRed_I (clause_groundings premise\<^sub>1 \<union> clause_groundings premise\<^sub>2)"
       using Infer_not_GRed_I .
   qed(auto)
@@ -1518,10 +1521,10 @@ proof-
   then obtain conclusion' where 
     superposition: "superposition premise\<^sub>2 premise\<^sub>1 conclusion'" and
     inference_groundings: 
-    "Infer [to_ground_clause (premise\<^sub>2 \<cdot> \<rho>\<^sub>2 \<cdot> \<theta>), to_ground_clause (premise\<^sub>1 \<cdot> \<rho>\<^sub>1 \<cdot> \<theta>)]
-        (to_ground_clause (conclusion' \<cdot> \<theta>)) \<in> 
+    "Infer [to_ground_clause (premise\<^sub>2 \<cdot> \<rho>\<^sub>2 \<cdot> \<gamma>), to_ground_clause (premise\<^sub>1 \<cdot> \<rho>\<^sub>1 \<cdot> \<gamma>)]
+        (to_ground_clause (conclusion' \<cdot> \<gamma>)) \<in> 
         inference_groundings (Infer [premise\<^sub>2, premise\<^sub>1] conclusion')" and  
-    conclusion'_conclusion: "conclusion' \<cdot> \<theta> = conclusion \<cdot> \<theta>"
+    conclusion'_conclusion: "conclusion' \<cdot> \<gamma> = conclusion \<cdot> \<gamma>"
     by metis
 
   let ?\<iota> = "Infer [premise\<^sub>2, premise\<^sub>1] conclusion'"
@@ -1575,26 +1578,26 @@ lemma for_all_elements_exists_f_implies_f_exists_for_all_elements:
 
 lemma necessary_select\<^sub>G_exists:
   obtains select\<^sub>G where 
-    "\<forall>premise\<^sub>G \<in> \<Union>(clause_groundings ` premises). \<exists>premise \<theta>. 
-          premise \<cdot> \<theta> = to_clause premise\<^sub>G 
-        \<and> select\<^sub>G premise\<^sub>G = to_ground_clause ((sel premise) \<cdot> \<theta>)
+    "\<forall>premise\<^sub>G \<in> \<Union>(clause_groundings ` premises). \<exists>premise \<gamma>. 
+          premise \<cdot> \<gamma> = to_clause premise\<^sub>G 
+        \<and> select\<^sub>G premise\<^sub>G = to_ground_clause ((sel premise) \<cdot> \<gamma>)
         \<and> premise \<in> premises" 
     "is_select_grounding sel select\<^sub>G"
 proof-
   let ?premise_groundings = "\<Union>(clause_groundings ` premises)"
 
-  have select\<^sub>G_exists_for_premises: "\<forall>premise\<^sub>G \<in> ?premise_groundings. \<exists>select\<^sub>G premise \<theta>.
-          premise \<cdot> \<theta> = to_clause premise\<^sub>G 
-        \<and> select\<^sub>G premise\<^sub>G = to_ground_clause ((sel premise) \<cdot> \<theta>)
+  have select\<^sub>G_exists_for_premises: "\<forall>premise\<^sub>G \<in> ?premise_groundings. \<exists>select\<^sub>G premise \<gamma>.
+          premise \<cdot> \<gamma> = to_clause premise\<^sub>G 
+        \<and> select\<^sub>G premise\<^sub>G = to_ground_clause ((sel premise) \<cdot> \<gamma>)
         \<and> premise \<in> premises"
     unfolding clause_groundings_def
     by fastforce
 
   obtain select\<^sub>G_on_premise_groundings where 
-    select\<^sub>G_on_premise_groundings: "\<forall>premise\<^sub>G \<in>?premise_groundings. \<exists>\<theta> premise. 
-        premise \<cdot> \<theta> = to_clause premise\<^sub>G 
-      \<and> select\<^sub>G_on_premise_groundings (to_ground_clause (premise \<cdot> \<theta>)) = 
-          to_ground_clause ((sel premise) \<cdot> \<theta>)
+    select\<^sub>G_on_premise_groundings: "\<forall>premise\<^sub>G \<in>?premise_groundings. \<exists>\<gamma> premise. 
+        premise \<cdot> \<gamma> = to_clause premise\<^sub>G 
+      \<and> select\<^sub>G_on_premise_groundings (to_ground_clause (premise \<cdot> \<gamma>)) = 
+          to_ground_clause ((sel premise) \<cdot> \<gamma>)
       \<and> premise \<in> premises"
     using 
       for_all_elements_exists_f_implies_f_exists_for_all_elements[OF select\<^sub>G_exists_for_premises]
@@ -1623,9 +1626,9 @@ lemma (in first_order_superposition_calculus) ground_instances:
     "is_grounding select\<^sub>G"
 proof-
   obtain select\<^sub>G where   
-    select\<^sub>G': "\<forall>premise\<^sub>G \<in> \<Union>(clause_groundings ` premises). \<exists>\<theta> premise. 
-          premise \<cdot> \<theta> = to_clause premise\<^sub>G 
-        \<and> to_clause (select\<^sub>G (to_ground_clause (premise \<cdot> \<theta>))) = (select premise) \<cdot> \<theta>
+    select\<^sub>G': "\<forall>premise\<^sub>G \<in> \<Union>(clause_groundings ` premises). \<exists>\<gamma> premise. 
+          premise \<cdot> \<gamma> = to_clause premise\<^sub>G 
+        \<and> to_clause (select\<^sub>G (to_ground_clause (premise \<cdot> \<gamma>))) = (select premise) \<cdot> \<gamma>
         \<and> premise \<in> premises" and
     "is_grounding select\<^sub>G" 
     using necessary_select\<^sub>G_exists
